@prefix : <http://www.sirma.com/ontologies/2014/05/hrConfiguration#> .
@prefix dc: <http://purl.org/dc/elements/1.1/> .
@prefix emf: <http://ittruse.ittbg.com/ontology/enterpriseManagementFramework#> .
@prefix hrc: <http://www.sirma.com/ontologies/2014/05/hrConfiguration#> .
@prefix owl: <http://www.w3.org/2002/07/owl#> .
@prefix rdf: <http://www.w3.org/1999/02/22-rdf-syntax-ns#> .
@prefix xml: <http://www.w3.org/XML/1998/namespace> .
@prefix xsd: <http://www.w3.org/2001/XMLSchema#> .
@prefix ptop: <http://www.ontotext.com/proton/protontop#> .
@prefix rdfs: <http://www.w3.org/2000/01/rdf-schema#> .
@prefix skos: <http://www.w3.org/2004/02/skos/core#> .
@prefix dcterms: <http://purl.org/dc/terms/> .
@base <http://www.sirma.com/ontologies/2014/05/hrConfiguration> .

<http://www.sirma.com/ontologies/2014/05/hrConfiguration> rdf:type owl:Ontology ;
                                                          
                                                          rdfs:label "Human Resources Management Ontology"@en ;
                                                          
                                                          dcterms:creator "Lidiya Dimitrova" ;
                                                          
                                                          skos:definition "Human Resources Management Ontology"@en ;
                                                          
                                                          dc:subject "Human Resources Management Ontology"@en ;
                                                          
                                                          owl:versionInfo "v 0.1" ;
                                                          
                                                          owl:imports <http://ittruse.ittbg.com/ontology/enterpriseManagementFramework> .


#################################################################
#
#    Annotation properties
#
#################################################################


###  http://purl.org/dc/terms/creator

dcterms:creator rdf:type owl:AnnotationProperty .





#################################################################
#
#    Object Properties
#
#################################################################


###  http://www.sirma.com/ontologies/2014/05/hrConfiguration#hasCandidate

:hasCandidate rdf:type owl:ObjectProperty ;
              
              rdfs:label "has candidate"@en ;
              
              dc:creator "Lidiya Dimitrova" ;
              
              skos:definition "Represents that the job position has a candidate."@en ;
              
              rdfs:range ptop:Person ;
              
              rdfs:domain :JobPosition ;
              
              owl:inverseOf :isCandidate .



###  http://www.sirma.com/ontologies/2014/05/hrConfiguration#hasCompetence

:hasCompetence rdf:type owl:ObjectProperty ;
               
               rdfs:label "has competence" ;
               
               dc:creator "Lidiya Dimitrova" ;
               
               skos:definition "Represents that person has a qualification." ;
               
               rdfs:domain ptop:Person ;
               
               rdfs:range :Competency .



###  http://www.sirma.com/ontologies/2014/05/hrConfiguration#hasContractWith

:hasContractWith rdf:type owl:ObjectProperty ;
                 
                 rdfs:label "has contract with" ;
                 
                 dc:creator "Lidiya Dimitrova" ;
                 
                 skos:definition "Reresents that the employee and the company have signed an employment contract."@en ;
                 
                 rdfs:range ptop:Agent ;
                 
                 rdfs:domain ptop:Agent ;
                 
                 owl:inverseOf :hasContractWith .



###  http://www.sirma.com/ontologies/2014/05/hrConfiguration#hasEmployee

:hasEmployee rdf:type owl:ObjectProperty ;
             
             rdfs:label "has employee" ;
             
             skos:definition "Represents the relation between the employee and the company employer." ;
             
             dc:creator "Lidiya Dimitrova" ;
             
             rdfs:domain emf:Company ;
             
             rdfs:range ptop:Person .



###  http://www.sirma.com/ontologies/2014/05/hrConfiguration#hasSubsidiary

:hasSubsidiary rdf:type owl:ObjectProperty ;
               
               rdfs:label "has subsidiary" ;
               
               dc:creator "Lidiya Dimitrova" ;
               
               skos:definition """Represents that a company has subsidiary company.
A subsidiary, subsidiary company, daughter company, or sister companies a company that is completely or partly owned by another corporation that owns more than half of the subsidiary's stock, and which normally acts as a holding corporation which at least partly or (when as) a parent corporation, wholly controls the activities and policies of the daughter corporation"""@en ;
               
               rdfs:domain emf:Company ;
               
               rdfs:range emf:Company .



###  http://www.sirma.com/ontologies/2014/05/hrConfiguration#isCandidate

:isCandidate rdf:type owl:ObjectProperty ;
             
             rdfs:label "is candidate"@en ;
             
             dc:creator "Lidiya Dimitrova" ;
             
             skos:definition "Represents that a person is candidate for a job position."@en ;
             
             rdfs:domain ptop:Person ;
             
             rdfs:range :JobPosition .



###  http://www.sirma.com/ontologies/2014/05/hrConfiguration#isCompetenceOf

:isCompetenceOf rdf:type owl:ObjectProperty ;
                
                rdfs:label "is competence of" ;
                
                dc:creator "Lidiya Dimitrova" ;
                
                skos:definition "Represents that person has a qualification." ;
                
                rdfs:range ptop:Person ;
                
                rdfs:domain :Competency ;
                
                owl:inverseOf :hasCompetence .



###  http://www.sirma.com/ontologies/2014/05/hrConfiguration#isEmployeeOf

:isEmployeeOf rdf:type owl:ObjectProperty ;
              
              rdfs:label "is employee of" ;
              
              dc:creator "Lidiya Dimitrova" ;
              
              skos:definition "Represents the relation between the employee and the company employer."@en ;
              
              rdfs:range emf:Company ;
              
              rdfs:domain ptop:Person ;
              
              owl:inverseOf :hasEmployee .



###  http://www.sirma.com/ontologies/2014/05/hrConfiguration#isOfferedBy

:isOfferedBy rdf:type owl:ObjectProperty ;
             
             rdfs:label "is offered by" ;
             
             dc:creator "Lidiya Dimitrova" ;
             
             skos:definition "Each job position is offered by a Company."@en ;
             
             rdfs:range emf:Company ;
             
             rdfs:domain :JobPosition ;
             
             owl:inverseOf :offersJobPosition .



###  http://www.sirma.com/ontologies/2014/05/hrConfiguration#isRequiredCompetenceFor

:isRequiredCompetenceFor rdf:type owl:ObjectProperty ;
                         
                         rdfs:label "is required competence for" ;
                         
                         dc:creator "Lidiya Dimitrova" ;
                         
                         skos:definition "Represents that a job possiton requires a qualification."@en ;
                         
                         rdfs:domain :Competency ;
                         
                         rdfs:range :JobPosition ;
                         
                         owl:inverseOf :requiresCompetence .



###  http://www.sirma.com/ontologies/2014/05/hrConfiguration#isSubsidiary

:isSubsidiary rdf:type owl:ObjectProperty ;
              
              rdfs:label "is subsidiary" ;
              
              dc:creator "Lidiya Dimitrova" ;
              
              skos:definition """Represents that a company is subsidiary company to other company.
A subsidiary, subsidiary company, daughter company, or sister companies a company that is completely or partly owned by another corporation that owns more than half of the subsidiary's stock, and which normally acts as a holding corporation which at least partly or (when as) a parent corporation, wholly controls the activities and policies of the daughter corporation"""@en ;
              
              rdfs:domain emf:Company ;
              
              rdfs:range emf:Company ;
              
              owl:inverseOf :hasSubsidiary .



###  http://www.sirma.com/ontologies/2014/05/hrConfiguration#offersJobPosition

:offersJobPosition rdf:type owl:ObjectProperty ;
                   
                   rdfs:label "offers job position" ;
                   
                   dc:creator "Lidiya Dimitrova" ;
                   
                   skos:definition "Represents the relation between Company and the job offers made by this Company."@en ;
                   
                   rdfs:domain emf:Company ;
                   
                   rdfs:range :JobPosition .



###  http://www.sirma.com/ontologies/2014/05/hrConfiguration#requiresCompetence

:requiresCompetence rdf:type owl:ObjectProperty ;
                    
                    rdfs:label "requires competence" ;
                    
                    dc:creator "Lidiya Dimitrova" ;
                    
                    skos:definition "Represents that a job possiton requires a qualification."@en ;
                    
                    rdfs:range :Competency ;
                    
                    rdfs:domain :JobPosition .





#################################################################
#
#    Data properties
#
#################################################################


###  http://www.sirma.com/ontologies/2014/05/hrConfiguration#contractDate

:contractDate rdf:type owl:DatatypeProperty ;
              
              rdfs:label "Contract date"@en ;
              
              dc:creator "Lidiya Dimitrova" ;
              
              skos:definition "The date a new employee has signed a contract with the employeer."@en ;
              
              rdfs:domain ptop:Person ;
              
              rdfs:range xsd:dateTime .



###  http://www.sirma.com/ontologies/2014/05/hrConfiguration#dateOfEntry

:dateOfEntry rdf:type owl:DatatypeProperty ;
             
             rdfs:label "Date of entry"@en ;
             
             dc:creator "Lidiya Dimitrova" ;
             
             skos:definition "The date a new employee starts his/her service of the employer."@en ;
             
             rdfs:domain ptop:Person ;
             
             rdfs:range xsd:dateTime .



###  http://www.sirma.com/ontologies/2014/05/hrConfiguration#drivingLicense

:drivingLicense rdf:type owl:DatatypeProperty ;
                
                rdfs:label "Driving License"@en ;
                
                dcterms:creator "Lidiya Dimitrova" ;
                
                skos:definition "Official permission for someone to drive a car, received after passing a driving test, or a document showing this"@en .



###  http://www.sirma.com/ontologies/2014/05/hrConfiguration#education

:education rdf:type owl:DatatypeProperty ;
           
           rdfs:label "Education"@en ;
           
           dc:creator "Lidiya Dimitrova" ;
           
           skos:definition "A degree, level, or kind of schooling: a university education. "@en .



###  http://www.sirma.com/ontologies/2014/05/hrConfiguration#language

:language rdf:type owl:DatatypeProperty ;
          
          rdfs:label "Language" ;
          
          skos:definition "Language is the human capacity for acquiring and using complex systems of communication, and a language is any specific example of such a system."@en ;
          
          dc:creator "Lidiya Dimitrova" .



###  http://www.sirma.com/ontologies/2014/05/hrConfiguration#location

:location rdf:type owl:DatatypeProperty ;
          
          rdfs:label "Location"@en ;
          
          skos:definition "A place or position."@en ;
          
          dc:creator "Lidiya Dimitrova" .



###  http://www.sirma.com/ontologies/2014/05/hrConfiguration#occupation

:occupation rdf:type owl:DatatypeProperty ;
            
            rdfs:label "Occupation"@en ;
            
            dc:creator "Lidiya Dimitrova"@en ;
            
            skos:definition "Usual or principal business, calling, trade, or work a person is engaged in earning a living."@en .



###  http://www.sirma.com/ontologies/2014/05/hrConfiguration#personType

:personType rdf:type owl:DatatypeProperty ;
            
            rdfs:label "Person type"@en ;
            
            dc:creator "Lidiya Dimitrova" ;
            
            skos:definition "Type of person: Candidate, Employee" ;
            
            rdfs:domain ptop:Person .





#################################################################
#
#    Classes
#
#################################################################


###  http://www.sirma.com/ontologies/2014/05/hrConfiguration#Competency

:Competency rdf:type owl:Class ;
            
            rdfs:label "Competency"@en ;
            
            rdfs:subClassOf :HRObjects ;
            
            skos:definition "Competency: The combination of observable and measurable knowledge, skills, abilities and personal attributes that contribute to enhanced employee performance and ultimately result in organizational success."@en ;
            
            dc:creator "Lidiya Dimitrova" .



###  http://www.sirma.com/ontologies/2014/05/hrConfiguration#HRObjects

:HRObjects rdf:type owl:Class ;
           
           rdfs:label "HR Objects"@en ;
           
           rdfs:subClassOf emf:DomainObject ;
           
           skos:definition """Human resource (HR) object main class for every ontology that extends the current.

This class is the parent class for all specific for the HR domain objects.


"""@en ;
           
           dc:creator "Lidiya Dimitrova" .



###  http://www.sirma.com/ontologies/2014/05/hrConfiguration#HardSkill

:HardSkill rdf:type owl:Class ;
           
           rdfs:label "Hard skill"@en ;
           
           rdfs:subClassOf :Competency ;
           
           emf:isSearchable "true"^^xsd:boolean ;
           
           emf:isPartOfObjectLibrary "true"^^xsd:boolean ;
           
           dc:creator "Lidiya Dimitrova" ;
           
           skos:definition """Hard skills are specific, teachable abilities that may be required in a given context, such as a job or university application.

Examples of hard skills include:
- facility with spreadsheets
- typing
- proficiency with software applications
- operating machinery
- proficiency in a foreign language
- calculus
- a degree or certificate
- typing speed
"""@en .



###  http://www.sirma.com/ontologies/2014/05/hrConfiguration#Individual

:Individual rdf:type owl:Class ;
            
            rdfs:label "Person"@en ;
            
            rdfs:subClassOf ptop:Person ,
                            :HRObjects ;
            
            emf:isSearchable "true"^^xsd:boolean ;
            
            emf:isPartOfObjectLibrary "true"^^xsd:boolean ;
            
            dcterms:creator "Lidiya Dimitrova" ;
            
            skos:definition "a person"@en .



###  http://www.sirma.com/ontologies/2014/05/hrConfiguration#JobPosition

:JobPosition rdf:type owl:Class ;
             
             rdfs:label "Job Position"@en ;
             
             rdfs:subClassOf :HRObjects ;
             
             emf:isSearchable "true"^^xsd:boolean ;
             
             emf:isPartOfObjectLibrary "true"^^xsd:boolean ;
             
             dc:creator "Lidiya Dimitrova" ;
             
             skos:definition "Represents a job description (qualifications and skills the applicant should meet for a certain job position)."@en .



###  http://www.sirma.com/ontologies/2014/05/hrConfiguration#SoftSkill

:SoftSkill rdf:type owl:Class ;
           
           rdfs:label "Soft skill"@en ;
           
           rdfs:subClassOf :Competency ;
           
           emf:isPartOfObjectLibrary "true"^^xsd:boolean ;
           
           emf:isSearchable "true"^^xsd:boolean ;
           
           dc:creator "Lidiya Dimitrova" ;
           
           skos:definition "Soft skills is a term often associated with a person's \"EQ\" (Emotional Intelligence Quotient), the cluster of personality traits, social graces, communication, language, personal habits, friendliness, and optimism that characterize relationships with other people."@en .





#################################################################
#
#    Annotations
#
#################################################################


emf:Customer emf:isPartOfObjectLibrary "true"^^xsd:boolean .




###  Generated by the OWL API (version 3.4.2) http://owlapi.sourceforge.net

