@prefix : <http://www.semanticweb.org/owl/owlapi/turtle#> .
@prefix dc: <http://purl.org/dc/elements/1.1/> .
@prefix chd: <http://www.sirma.com/ontologies/2013/10/culturalHeritageDomain#> .
@prefix emf: <http://ittruse.ittbg.com/ontology/enterpriseManagementFramework#> .
@prefix owl: <http://www.w3.org/2002/07/owl#> .
@prefix rdf: <http://www.w3.org/1999/02/22-rdf-syntax-ns#> .
@prefix xml: <http://www.w3.org/XML/1998/namespace> .
@prefix xsd: <http://www.w3.org/2001/XMLSchema#> .
@prefix rdfs: <http://www.w3.org/2000/01/rdf-schema#> .
@prefix skos: <http://www.w3.org/2004/02/skos/core#> .
@prefix dcterms: <http://purl.org/dc/terms/> .
@base <http://www.sirma.com/ontologies/2013/10/culturalHeritageDomain> .

<http://www.sirma.com/ontologies/2013/10/culturalHeritageDomain> rdf:type owl:Ontology ;
                                                                 
                                                                 skos:definition "Cultural heritage domain model for Conservation Space project"@en ;
                                                                 
                                                                 dc:creator "Kiril Penev"@en ;
                                                                 
                                                                 owl:imports <http://ittruse.ittbg.com/ontology/enterpriseManagementFramework> .


#################################################################
#
#    Annotation properties
#
#################################################################


###  http://purl.org/dc/terms/description

dcterms:description rdf:type owl:AnnotationProperty .





#################################################################
#
#    Object Properties
#
#################################################################


###  http://www.sirma.com/ontologies/2013/10/culturalHeritageDomain#accordingToProposal

chd:accordingToProposal rdf:type owl:ObjectProperty ;
                        
                        rdfs:label "According to proposal"@en ;
                        
                        emf:isSearchable "true"^^xsd:boolean ;
                        
                        dc:creator "Kiril Penev"@en ;
                        
                        skos:definition "The proposal treatment on which this treatment is based on"@en ;
                        
                        rdfs:domain chd:ConservationTreatment ;
                        
                        rdfs:range chd:ConservationTreatment .



###  http://www.sirma.com/ontologies/2013/10/culturalHeritageDomain#bookCoverCondition

chd:bookCoverCondition rdf:type owl:ObjectProperty ;
                       
                       rdfs:label "book cover condition"@en ;
                       
                       skos:definition "Description of Book cover condition"@en ;
                       
                       dc:creator "Kiril Penev"@en ;
                       
                       rdfs:subPropertyOf chd:condition .



###  http://www.sirma.com/ontologies/2013/10/culturalHeritageDomain#bookCoverConstruction

chd:bookCoverConstruction rdf:type owl:ObjectProperty ;
                          
                          rdfs:label "book cover construction"@en ;
                          
                          skos:definition " Book cover construction description"@en ;
                          
                          dc:creator "Kiril Penev"@en ;
                          
                          rdfs:subPropertyOf chd:construction .



###  http://www.sirma.com/ontologies/2013/10/culturalHeritageDomain#condition

chd:condition rdf:type owl:ObjectProperty ;
              
              rdfs:label "condition"@en ;
              
              skos:definition " Condigion relation"@en ;
              
              dc:creator "Kiril Penev"@en .



###  http://www.sirma.com/ontologies/2013/10/culturalHeritageDomain#construction

chd:construction rdf:type owl:ObjectProperty ;
                 
                 rdfs:label "construction"@en ;
                 
                 skos:definition "Construction relation"@en ;
                 
                 dc:creator "Kiril Penev"@en ;
                 
                 rdfs:subPropertyOf owl:topObjectProperty .



###  http://www.sirma.com/ontologies/2013/10/culturalHeritageDomain#duringTreatmentExamination

chd:duringTreatmentExamination rdf:type owl:ObjectProperty ;
                               
                               rdfs:label "during treatment examination"@en ;
                               
                               skos:definition "Examination that is made during the treatment"@en ;
                               
                               dc:creator "Kiril Penev"@en ;
                               
                               rdfs:range chd:ConservationExamination ;
                               
                               rdfs:domain chd:ConservationTreatment .



###  http://www.sirma.com/ontologies/2013/10/culturalHeritageDomain#dyes

chd:dyes rdf:type owl:ObjectProperty ;
         
         rdfs:label "dyes"@en ;
         
         dc:creator "Kiril Penev"@en ;
         
         skos:definition "Textile Dyes description"@en .



###  http://www.sirma.com/ontologies/2013/10/culturalHeritageDomain#frameConstruction

chd:frameConstruction rdf:type owl:ObjectProperty ;
                      
                      rdfs:label "frame construction"@en ;
                      
                      dc:creator "Kiril Penev"@en ;
                      
                      skos:definition "Method of frame construction"@en ;
                      
                      rdfs:subPropertyOf chd:construction .



###  http://www.sirma.com/ontologies/2013/10/culturalHeritageDomain#frameFinishMaterial

chd:frameFinishMaterial rdf:type owl:ObjectProperty ;
                        
                        rdfs:label "frame finish material"@en ;
                        
                        dc:creator "Kiril Penev"@en ;
                        
                        skos:definition "Type of frame finishing material. E.g. shellac, brush applied"@en .



###  http://www.sirma.com/ontologies/2013/10/culturalHeritageDomain#frameMaterial

chd:frameMaterial rdf:type owl:ObjectProperty ;
                  
                  rdfs:label "frame material"@en ;
                  
                  dc:creator "Kiril Penev"@en ;
                  
                  skos:definition "Type of frame material"@en .



###  http://www.sirma.com/ontologies/2013/10/culturalHeritageDomain#hasActionList

chd:hasActionList rdf:type owl:ObjectProperty ;
                  
                  rdfs:label "has action list"@en ;
                  
                  emf:isSearchable "true"^^xsd:boolean ;
                  
                  dc:creator "Kiril Penev"@en ;
                  
                  skos:definition "List with Conservation Actions that will be executed during the treatment"@en ;
                  
                  rdfs:domain chd:ConservationTreatment ;
                  
                  rdfs:range chd:ConservationTreatmentAction .



###  http://www.sirma.com/ontologies/2013/10/culturalHeritageDomain#hasMark

chd:hasMark rdf:type owl:ObjectProperty ;
            
            rdfs:label "has mark"@en ;
            
            skos:definition "Description of any marks not related to the image such notations or marks made by a processes "@en ;
            
            dc:creator "Kiril Penev"@en ;
            
            rdfs:domain chd:CulturalObject ;
            
            rdfs:range chd:Mark .



###  http://www.sirma.com/ontologies/2013/10/culturalHeritageDomain#hasMounting

chd:hasMounting rdf:type owl:ObjectProperty ;
                
                rdfs:label "hasMounting"@en ;
                
                skos:definition "General description of the mounting of the cultural object"@en ;
                
                dc:creator "Kiril Penev"@en ;
                
                rdfs:range emf:DatedConcept ;
                
                rdfs:domain chd:CulturalObject .



###  http://www.sirma.com/ontologies/2013/10/culturalHeritageDomain#hasPerformer

chd:hasPerformer rdf:type owl:ObjectProperty ;
                 
                 rdfs:label "has performer"@en ;
                 
                 dc:creator "Kiril Penev"@en ;
                 
                 skos:definition "The relation between a happenning and the agent responsbile for executing/performing it. Usualy the performer of a happenning is a user with specific role (role of executor/performer)."@en ;
                 
                 rdfs:range <http://www.ontotext.com/proton/protontop#Agent> .



###  http://www.sirma.com/ontologies/2013/10/culturalHeritageDomain#hasPlacement

chd:hasPlacement rdf:type owl:ObjectProperty ;
                 
                 rdfs:label "has placement"@en ;
                 
                 skos:definition " The relative location of a Mark on the cultural object."@en ;
                 
                 dc:creator "Kiril Penev"@en ;
                 
                 rdfs:domain chd:Mark .



###  http://www.sirma.com/ontologies/2013/10/culturalHeritageDomain#imageLayerCondition

chd:imageLayerCondition rdf:type owl:ObjectProperty ;
                        
                        rdfs:label "image layer condition"@en ;
                        
                        skos:definition " Condition of material that the image is made of"@en ;
                        
                        dc:creator "Kiril Penev"@en ;
                        
                        rdfs:subPropertyOf chd:condition .



###  http://www.sirma.com/ontologies/2013/10/culturalHeritageDomain#imageLayerConstruction

chd:imageLayerConstruction rdf:type owl:ObjectProperty ;
                           
                           rdfs:label "image layer construction"@en ;
                           
                           dc:creator "Kiril Penev"@en ;
                           
                           skos:definition "Type of material that the image is made of"@en ;
                           
                           rdfs:subPropertyOf chd:construction .



###  http://www.sirma.com/ontologies/2013/10/culturalHeritageDomain#methodOfConstruction

chd:methodOfConstruction rdf:type owl:ObjectProperty ;
                         
                         rdfs:label "method of construction"@en ;
                         
                         skos:definition "Detailed description of the construction of a cultural object."@en ;
                         
                         dc:creator "Kiril Penev"@en .



###  http://www.sirma.com/ontologies/2013/10/culturalHeritageDomain#methodOfUpholstery

chd:methodOfUpholstery rdf:type owl:ObjectProperty ;
                       
                       rdfs:label "method of upholstery"@en ;
                       
                       skos:definition "Detailed description of the method of upholstery of a cultural object."@en ;
                       
                       dc:creator "Kiril Penev"@en .



###  http://www.sirma.com/ontologies/2013/10/culturalHeritageDomain#mountingCondition

chd:mountingCondition rdf:type owl:ObjectProperty ;
                      
                      rdfs:label "mounting condition"@en ;
                      
                      skos:definition " Condition of the mount on which the photograph is mounted or housed"@en ;
                      
                      dc:creator "Kiril Penev"@en ;
                      
                      rdfs:subPropertyOf chd:condition .



###  http://www.sirma.com/ontologies/2013/10/culturalHeritageDomain#mountingConstruction

chd:mountingConstruction rdf:type owl:ObjectProperty ;
                         
                         rdfs:label "mounting construction"@en ;
                         
                         skos:definition "Description of how the photograph is mounted or housed"@en ;
                         
                         dc:creator "Kiril Penev"@en ;
                         
                         rdfs:subPropertyOf chd:construction .



###  http://www.sirma.com/ontologies/2013/10/culturalHeritageDomain#paintLayersCondition

chd:paintLayersCondition rdf:type owl:ObjectProperty ;
                         
                         rdfs:label "paint layers condition"@en ;
                         
                         skos:definition " Technical description of the paint layer or design condition"@en ;
                         
                         dc:creator "Kiril Penev"@en ;
                         
                         rdfs:subPropertyOf chd:condition .



###  http://www.sirma.com/ontologies/2013/10/culturalHeritageDomain#paintLayersConstruction

chd:paintLayersConstruction rdf:type owl:ObjectProperty ;
                            
                            rdfs:label "paint layers construction"@en ;
                            
                            dc:creator "Kiril Penev"@en ;
                            
                            skos:definition "Technical description of the paint layer or design construction"@en ;
                            
                            rdfs:subPropertyOf chd:construction .



###  http://www.sirma.com/ontologies/2013/10/culturalHeritageDomain#postTreatmentExamination

chd:postTreatmentExamination rdf:type owl:ObjectProperty ;
                             
                             rdfs:label "post treatment examination"@en ;
                             
                             skos:definition " Examination that is done after the treatment to identify the condition of the cultural object after the treatment"@en ;
                             
                             dc:creator "Kiril Penev"@en ;
                             
                             rdfs:range chd:ConservationExamination ;
                             
                             rdfs:domain chd:ConservationTreatment .



###  http://www.sirma.com/ontologies/2013/10/culturalHeritageDomain#preTreatmentExamination

chd:preTreatmentExamination rdf:type owl:ObjectProperty ;
                            
                            rdfs:label "pre treatment examination"@en ;
                            
                            skos:definition " Examination that is done before the treatement to identify the condition of the cultural object and what treatments are needed"@en ;
                            
                            dc:creator "Kiril Penev"@en ;
                            
                            rdfs:range chd:ConservationExamination ;
                            
                            rdfs:domain chd:ConservationTreatment ;
                            
                            rdfs:subPropertyOf owl:topObjectProperty .



###  http://www.sirma.com/ontologies/2013/10/culturalHeritageDomain#sizingAndGroundCondition

chd:sizingAndGroundCondition rdf:type owl:ObjectProperty ;
                             
                             rdfs:label "sizing and ground condition"@en ;
                             
                             skos:definition " Technical description of the sizing and ground condition"@en ;
                             
                             dc:creator "Kiril Penev"@en ;
                             
                             rdfs:subPropertyOf chd:condition .



###  http://www.sirma.com/ontologies/2013/10/culturalHeritageDomain#sizingAndGroundConstriuction

chd:sizingAndGroundConstriuction rdf:type owl:ObjectProperty ;
                                 
                                 rdfs:label "sizing and ground constriuction"@en ;
                                 
                                 dc:creator "Kiril Penev"@en ;
                                 
                                 skos:definition "Technical description of the sizing and ground construction"@en ;
                                 
                                 rdfs:subPropertyOf chd:construction .



###  http://www.sirma.com/ontologies/2013/10/culturalHeritageDomain#substrateCondition

chd:substrateCondition rdf:type owl:ObjectProperty ;
                       
                       rdfs:label "substrate condition"@en ;
                       
                       skos:definition " Substrate condition "@en ;
                       
                       dc:creator "Kiril Penev"@en ;
                       
                       rdfs:subPropertyOf chd:condition .



###  http://www.sirma.com/ontologies/2013/10/culturalHeritageDomain#substrateConstruction

chd:substrateConstruction rdf:type owl:ObjectProperty ;
                          
                          rdfs:label "substrate construction"@en ;
                          
                          dc:creator "Kiril Penev"@en ;
                          
                          skos:definition "The primary structural material used in the object; the decorative/presentation surface sits on this material"@en ;
                          
                          rdfs:subPropertyOf chd:construction .



###  http://www.sirma.com/ontologies/2013/10/culturalHeritageDomain#supportCondition

chd:supportCondition rdf:type owl:ObjectProperty ;
                     
                     rdfs:label "support condition"@en ;
                     
                     dc:creator "Kiril Penev"@en ;
                     
                     skos:definition "Technical description of the support(s) condition"@en ;
                     
                     rdfs:subPropertyOf chd:condition .



###  http://www.sirma.com/ontologies/2013/10/culturalHeritageDomain#supportConstruction

chd:supportConstruction rdf:type owl:ObjectProperty ;
                        
                        rdfs:label "support construction"@en ;
                        
                        dc:creator "Kiril Penev"@en ;
                        
                        skos:definition "Technical description of the support(s) construction"@en ;
                        
                        rdfs:subPropertyOf chd:construction .



###  http://www.sirma.com/ontologies/2013/10/culturalHeritageDomain#surfaceCoatingCondition

chd:surfaceCoatingCondition rdf:type owl:ObjectProperty ;
                            
                            rdfs:label "surface coating condition"@en ;
                            
                            skos:definition "Detailed description of surface coating(s)' condition"@en ;
                            
                            dc:creator "Kiril Penev"@en ;
                            
                            rdfs:subPropertyOf chd:condition .



###  http://www.sirma.com/ontologies/2013/10/culturalHeritageDomain#surfaceCoatingConstruction

chd:surfaceCoatingConstruction rdf:type owl:ObjectProperty ;
                               
                               rdfs:label "surface coating construction"@en ;
                               
                               skos:definition "Detailed description of surface coating(s)"@en ;
                               
                               dc:creator "Kiril Penev"@en ;
                               
                               rdfs:subPropertyOf chd:construction .



###  http://www.sirma.com/ontologies/2013/10/culturalHeritageDomain#surfaceDescription

chd:surfaceDescription rdf:type owl:ObjectProperty ;
                       
                       rdfs:label "surface description"@en ;
                       
                       skos:definition "Detailed description of the surface of a cultural object."@en ;
                       
                       dc:creator "Kiril Penev"@en ;
                       
                       rdfs:subPropertyOf owl:topObjectProperty .



###  http://www.sirma.com/ontologies/2013/10/culturalHeritageDomain#upholsteryMaterial

chd:upholsteryMaterial rdf:type owl:ObjectProperty ;
                       
                       rdfs:label "upholstery material"@en ;
                       
                       skos:definition "Detailed description of the materials of upholstery of a cultural object."@en ;
                       
                       dc:creator "Kiril Penev"@en .



###  http://www.sirma.com/ontologies/2013/10/culturalHeritageDomain#usesMaterials

chd:usesMaterials rdf:type owl:ObjectProperty ;
                  
                  rdfs:label "uses materials"@en ;
                  
                  emf:isSearchable "true"^^xsd:boolean ;
                  
                  skos:definition "Describes the materials used during a treatment activity (such as conservation treatment actions)."@en ;
                  
                  dc:creator "Kiril Penev"@en .



###  http://www.sirma.com/ontologies/2013/10/culturalHeritageDomain#watermarkDescription

chd:watermarkDescription rdf:type owl:ObjectProperty ;
                         
                         rdfs:label "watermark description"@en ;
                         
                         skos:definition "Free text description of any watermarks evident in the paper/support"@en ;
                         
                         dc:creator "Kiril Penev"@en .



###  http://www.sirma.com/ontologies/2013/10/culturalHeritageDomain#weave

chd:weave rdf:type owl:ObjectProperty ;
          
          rdfs:label "weave"@en ;
          
          skos:definition "Description of textiles weave"@en ;
          
          dc:creator "Kiril Penev"@en .





#################################################################
#
#    Data properties
#
#################################################################


###  http://www.ontotext.com/proton/protontop#endTime

<http://www.ontotext.com/proton/protontop#endTime> rdfs:range xsd:dateTime .



###  http://www.ontotext.com/proton/protontop#startTime

<http://www.ontotext.com/proton/protontop#startTime> rdfs:range xsd:dateTime .



###  http://www.sirma.com/ontologies/2013/10/culturalHeritageDomain#accessionNumber

chd:accessionNumber rdf:type owl:DatatypeProperty ;
                       
                       rdfs:label "Accession Number"@en ;
                       
                       skos:definition "Accession Number of the instance"@en ;
                       
                       dc:creator "Kiril Penev"@en .



###  http://www.sirma.com/ontologies/2013/10/culturalHeritageDomain#basePhysicalDimensions

chd:basePhysicalDimensions rdf:type owl:DatatypeProperty ;
                       
                       rdfs:label "Base Physical Dimensions"@en ;
                       
                       skos:definition "Base Physical Dimensions of the Cultural object"@en ;
                       
                       dc:creator "Kiril Penev"@en .



###  http://www.sirma.com/ontologies/2013/10/culturalHeritageDomain#examinationPurpose

chd:examinationPurpose rdf:type owl:DatatypeProperty ;
                       
                       rdfs:label "Examination Purpose"@en ;
                       
                       skos:definition "Examination Purpose of the Case"@en ;
                       
                       dc:creator "Kiril Penev"@en ;
                       
                       rdfs:domain emf:Case .



###  http://www.sirma.com/ontologies/2013/10/culturalHeritageDomain#markContent

chd:markContent rdf:type owl:DatatypeProperty ;
                
                rdfs:label "mark content"@en ;
                
                skos:definition " Description of the mark"@en ;
                
                dc:creator "Kiril Penev"@en ;
                
                rdfs:domain chd:Mark .



###  http://www.sirma.com/ontologies/2013/10/culturalHeritageDomain#mountings

chd:mountings rdf:type owl:DatatypeProperty ;
              
              rdfs:label "mountings"@en ;
              
              skos:definition "General description of the mounting of the cultural object"@en ;
              
              dc:creator "Kiril Penev"@en ;
              
              rdfs:domain chd:CulturalObject .





#################################################################
#
#    Classes
#
#################################################################


###  http://www.sirma.com/ontologies/2013/10/culturalHeritageDomain#Book

chd:Book rdf:type owl:Class ;
         
         rdfs:label "Book"@en ;
         
         rdfs:subClassOf chd:CulturalObject ;
         
         emf:isPartOfObjectLibrary "true"^^xsd:boolean ;
         
         emf:isSearchable "true"^^xsd:boolean ;
         
         skos:definition "A set of written, printed, or blank pages fastened along one side and encased between protective covers."@en ;
         
         dc:creator "Kiril Penev"@en .



###  http://www.sirma.com/ontologies/2013/10/culturalHeritageDomain#BoundManuscript

chd:BoundManuscript rdf:type owl:Class ;
                    
                    rdfs:label "Bound Manuscript"@en ;
                    
                    rdfs:subClassOf chd:CulturalObject ;
                    
                    emf:isPartOfObjectLibrary "true"^^xsd:boolean ;
                    
                    emf:isSearchable "true"^^xsd:boolean ;
                    
                    skos:definition "Bound manuscript"@en ;
                    
                    dc:creator "Kiril Penev"@en .



###  http://www.sirma.com/ontologies/2013/10/culturalHeritageDomain#Condition

chd:Condition rdf:type owl:Class ;
              
              rdfs:label "Condition"@en ;
              
              rdfs:subClassOf skos:Concept ;
              
              dcterms:description "Information about the status of a cultural object, such as entirety, visible defects and marks, damage description, etc. "@en ;
              
              dc:creator "Kiril Penev"@en .



###  http://www.sirma.com/ontologies/2013/10/culturalHeritageDomain#ConservationActivity

chd:ConservationActivity rdf:type owl:Class ;
                         
                         rdfs:label "Conservation Activity"@en ;
                         
                         rdfs:subClassOf chd:CulturalActivity ;
                         
                         emf:isSearchable "true"^^xsd:boolean ;
                         
                         skos:definition "Activities that are connected with Conservation of a cultural Objects"@en ;
                         
                         dc:creator "Kiril Penev"@en .



###  http://www.sirma.com/ontologies/2013/10/culturalHeritageDomain#ConservationExamination

chd:ConservationExamination rdf:type owl:Class ;
                            
                            rdfs:label "Conservation Examination"@en ;
                            
                            rdfs:subClassOf chd:ConservationActivity ;
                            
                            emf:isSearchable "true"^^xsd:boolean ;
                            
                            skos:definition "Conservation examination is number of activities for gathering technical and conditional information for the cultural object. Examinations can be performed for a possible treatment, a possible change of the object`s location, for possible acquisition and etc."@en ;
                            
                            dc:creator "Kiril Penev"@en .



###  http://www.sirma.com/ontologies/2013/10/culturalHeritageDomain#ConservationExaminationAction

chd:ConservationExaminationAction rdf:type owl:Class ;
                                  
                                  rdfs:label "Conservation Examination Action"@en ;
                                  
                                  rdfs:subClassOf chd:ConservationExamination ;
                                  
                                  emf:isSearchable "true"^^xsd:boolean ;
                                  
                                  skos:definition "Conservation Examination Action is a single activity performed during examination of the cultural object. Such actions are documenting the construction, the condition of the object, photographing the object and etc."@en ;
                                  
                                  dc:creator "Kiril Penev"@en .



###  http://www.sirma.com/ontologies/2013/10/culturalHeritageDomain#ConservationTreatment

chd:ConservationTreatment rdf:type owl:Class ;
                          
                          rdfs:label "Conservation Treatment"@en ;
                          
                          rdfs:subClassOf chd:ConservationActivity ;
                          
                          emf:isSearchable "true"^^xsd:boolean ;
                          
                          skos:definition "Conservation Treatment is a list of actions that has the purpouse of restoring old or damaged cultural object to their original state."@en ;
                          
                          dc:creator "Kiril Penev"@en .



###  http://www.sirma.com/ontologies/2013/10/culturalHeritageDomain#ConservationTreatmentAction

chd:ConservationTreatmentAction rdf:type owl:Class ;
                                
                                rdfs:label "Conservation Treatment Action"@en ;
                                
                                rdfs:subClassOf chd:ConservationTreatment ;
                                
                                emf:isSearchable "true"^^xsd:boolean ;
                                
                                skos:definition "Conservation Treatment Action is a single activity that is performed in order to accomplish the restoration of a cultural object. Such actions are relining a painting, attaching a new canvas to the back, surface cleaning, filling and inpainting looses etc. "@en ;
                                
                                dc:creator "Kiril Penev"@en .



###  http://www.sirma.com/ontologies/2013/10/culturalHeritageDomain#CulturalActivity

chd:CulturalActivity rdf:type owl:Class ;
                     
                     rdfs:label "Cultural Activity"@en ;
                     
                     rdfs:subClassOf emf:Activity ;
                     
                     emf:isSearchable "true"^^xsd:boolean ;
                     
                     dc:creator "Kiril Penev"@en ;
                     
                     skos:definition "Main class for grouping Cultural activities"@en .



###  http://www.sirma.com/ontologies/2013/10/culturalHeritageDomain#CulturalEvent

chd:CulturalEvent rdf:type owl:Class ;
                  
                  rdfs:label "Cultural Event"@en ;
                  
                  rdfs:subClassOf <http://www.ontotext.com/proton/protontop#Event> ;
                  
                  emf:isSearchable "true"^^xsd:boolean ;
                  
                  dc:creator "Kiril Penev"@en ;
                  
                  skos:definition "Organized events such as art events, Exhibitions‎, Museum events and etc."@en .



###  http://www.sirma.com/ontologies/2013/10/culturalHeritageDomain#CulturalObject

chd:CulturalObject rdf:type owl:Class ;
                   
                   rdfs:label "Cultural Object"@en ;
                   
                   rdfs:subClassOf emf:DomainObject ;
                   
                   emf:isSearchable "true"^^xsd:boolean ;
                   
                   skos:definition "A cultural object is an object made by humans for a practical and/or spiritual purpose. Cultural object is involved in cultural activities"@en ;
                   
                   dc:creator "Kiril Penev"@en ;
                   
                   emf:definitionId "objectinstance"@en .



###  http://www.sirma.com/ontologies/2013/10/culturalHeritageDomain#Drawing

chd:Drawing rdf:type owl:Class ;
            
            rdfs:label "Drawing"@en ;
            
            rdfs:subClassOf chd:CulturalObject ;
            
            emf:isSearchable "true"^^xsd:boolean ;
            
            emf:isPartOfObjectLibrary "true"^^xsd:boolean ;
            
            skos:definition "Drawing is a form of visual art that makes use of any number of drawing instruments to mark a two-dimensional medium. Instruments used include graphite pencils, pen and ink, inked brushes, wax color pencils, crayons, charcoal, chalk, pastels, various kinds of erasers, markers, styluses, and various metals (such as silverpoint) (Wikipedia)"@en ;
            
            dc:creator "Kiril Penev"@en .



###  http://www.sirma.com/ontologies/2013/10/culturalHeritageDomain#Exhibition

chd:Exhibition rdf:type owl:Class ;
               
               rdfs:label "Exhibition"@en ;
               
               rdfs:subClassOf chd:CulturalEvent ;
               
               emf:isSearchable "true"^^xsd:boolean ;
               
               skos:definition "An exhibition, in the most general sense, is an organized presentation and display of a selection of items. In practice, exhibitions usually occur within museums, galleries and exhibition halls, and World's Fairs."@en ;
               
               dc:creator "Kiril Penev"@en .



###  http://www.sirma.com/ontologies/2013/10/culturalHeritageDomain#Furniture

chd:Furniture rdf:type owl:Class ;
              
              rdfs:label "Furniture"@en ;
              
              rdfs:subClassOf chd:CulturalObject ;
              
              emf:isPartOfObjectLibrary "true"^^xsd:boolean ;
              
              emf:isSearchable "true"^^xsd:boolean ;
              
              skos:definition "Furniture is the mass noun for the movable objects intended to support various human activities such as seating and sleeping. Furniture is also used to hold objects at a convenient height for work (as horizontal surfaces above the ground), or to store things. (Wikipedia)"@en ;
              
              dc:creator "Kiril Penev"@en .



###  http://www.sirma.com/ontologies/2013/10/culturalHeritageDomain#Inscription

chd:Inscription rdf:type owl:Class ;
                
                rdfs:label "Inscription"@en ;
                
                rdfs:subClassOf chd:CulturalObject ;
                
                dc:creator "Kiril Penev"@en ;
                
                skos:definition "Text carved on a wall or plaque, such as a memorial or gravestone."@en .



###  http://www.sirma.com/ontologies/2013/10/culturalHeritageDomain#Mark

chd:Mark rdf:type owl:Class ;
         
         rdfs:label "Mark"@en ;
         
         rdfs:subClassOf chd:CulturalObject ;
         
         emf:isSearchable "true"^^xsd:boolean ;
         
         skos:definition "Description of any marks not related to the image such notations or marks made by processes. "@en ;
         
         dc:creator "Kiril Penev"@en .



###  http://www.sirma.com/ontologies/2013/10/culturalHeritageDomain#MarkType

chd:MarkType rdf:type owl:Class ;
             
             rdfs:label "Mark Type"@en ;
             
             rdfs:subClassOf skos:Concept ;
             
             skos:definition "Information about the type of the mark on a cultural object."@en ;
             
             dc:creator "Kiril Penev"@en .



###  http://www.sirma.com/ontologies/2013/10/culturalHeritageDomain#Materials

chd:Materials rdf:type owl:Class ;
              
              rdfs:label "Materials"@en ;
              
              rdfs:subClassOf skos:Concept ;
              
              skos:definition "Description of used materials during a treatment activity."@en ;
              
              dc:creator "Kiril Penev"@en .



###  http://www.sirma.com/ontologies/2013/10/culturalHeritageDomain#Painting

chd:Painting rdf:type owl:Class ;
             
             rdfs:label "Painting"@en ;
             
             rdfs:subClassOf chd:CulturalObject ;
             
             emf:isSearchable "true"^^xsd:boolean ;
             
             emf:isPartOfObjectLibrary "true"^^xsd:boolean ;
             
             dc:creator "Kiril Penev"@en ;
             
             skos:definition "Painting is the practice of applying paint, pigment, color or other medium to a surface (support base). The medium is commonly applied to the base with a brush but other implements, such as knives, sponges, and airbrushes, can be used. In art, the term painting describes both the act and the result of the action. However, painting is also used outside of art as a common trade among craftsmen and builders. Paintings may have for their support such surfaces as walls, paper, canvas, wood, glass, lacquer, clay, leaf, copper or concrete, and may incorporate multiple other materials including sand, clay, paper, gold leaf as well as objects. (Wikipedia)"@en .



###  http://www.sirma.com/ontologies/2013/10/culturalHeritageDomain#Photograph

chd:Photograph rdf:type owl:Class ;
               
               rdfs:label "Photograph"@en ;
               
               rdfs:subClassOf chd:CulturalObject ;
               
               emf:isPartOfObjectLibrary "true"^^xsd:boolean ;
               
               emf:isSearchable "true"^^xsd:boolean ;
               
               skos:definition "A photograph or photo is an image created by light falling on a light-sensitive surface, usually photographic film or an electronic image such as a CCD or a CMOS chip. Most photographs are created using a camera, which uses a lens to focus the scene's visible wavelengths of light into a reproduction of what the human eye would see. (Wikipedia)"@en ;
               
               dc:creator "Kiril Penev"@en .



###  http://www.sirma.com/ontologies/2013/10/culturalHeritageDomain#Print

chd:Print rdf:type owl:Class ;
          
          rdfs:label "Print"@en ;
          
          rdfs:subClassOf chd:CulturalObject ;
          
          emf:isSearchable "true"^^xsd:boolean ;
          
          emf:isPartOfObjectLibrary "true"^^xsd:boolean ;
          
          skos:definition """A picture or design printed from a block or plate or copied from a painting by photography.
A piece of fabric or clothing with a decorative colored pattern or design printed on it."""@en ;
          
          dc:creator "Kiril Penev"@en .



###  http://www.sirma.com/ontologies/2013/10/culturalHeritageDomain#Sample

chd:Sample rdf:type owl:Class ;
           
           rdfs:label "Sample"@en ;
           
           rdfs:subClassOf chd:CulturalObject ;
           
           emf:isPartOfObjectLibrary "true"^^xsd:boolean ;
           
           emf:isSearchable "true"^^xsd:boolean ;
           
           dc:creator "Kiril Penev"@en ;
           
           skos:definition "Sample is a representative part or a single item from a larger whole or group especially when presented for inspection or shown as evidence of quality. Samples are taken from the cultural object to make additional scientiffic analysis on the used materials, technics and etc."@en .



###  http://www.sirma.com/ontologies/2013/10/culturalHeritageDomain#Sculpture

chd:Sculpture rdf:type owl:Class ;
              
              rdfs:label "Sculpture"@en ;
              
              rdfs:subClassOf chd:CulturalObject ;
              
              emf:isPartOfObjectLibrary "true"^^xsd:boolean ;
              
              emf:isSearchable "true"^^xsd:boolean ;
              
              dc:creator "Kiril Penev"@en ;
              
              skos:definition "Sculpture is the branch of the visual arts that operates in three dimensions, and one of the plastic arts. Durable sculptural processes originally used carving (the removal of material) and modelling (the addition of material, as clay), in stone, metal, ceramics, wood and other materials but, since modernism, shifts in sculptural process led to an almost complete freedom of materials and process. A wide variety of materials may be worked by removal such as carving, assembled by welding or modelling, or molded, or cast. (Wikipedia)"@en .



###  http://www.sirma.com/ontologies/2013/10/culturalHeritageDomain#Textiles

chd:Textiles rdf:type owl:Class ;
             
             rdfs:label "Textiles"@en ;
             
             rdfs:subClassOf chd:CulturalObject ;
             
             emf:isSearchable "true"^^xsd:boolean ;
             
             emf:isPartOfObjectLibrary "true"^^xsd:boolean ;
             
             skos:definition "A textile or cloth is a flexible woven material consisting of a network of natural or artificial fibres often referred to as thread or yarn. Yarn is produced by spinning raw fibres of wool, flax, cotton, or other material to produce long strands. Textiles are formed by weaving, knitting, crocheting, knotting, or pressing fibres together (felt). (Wikipedia)"@en ;
             
             dc:creator "Kiril Penev"@en .



###  http://www.sirma.com/ontologies/2013/10/culturalHeritageDomain#TreatmentActivity

chd:TreatmentActivity rdf:type owl:Class ;
                      
                      rdfs:label "Treatment Activity"@en ;
                      
                      rdfs:subClassOf skos:Concept ;
                      
                      skos:definition "Information about the activities included in one treatment operation - steps performed, executor, cultural object, etc."@en ;
                      
                      dc:creator "Kiril Penev"@en .



###  http://www.sirma.com/ontologies/2013/10/culturalHeritageDomain#TreatmentType

chd:TreatmentType rdf:type owl:Class ;
                  
                  rdfs:label "Treatment Type"@en ;
                  
                  rdfs:subClassOf skos:Concept ;
                  
                  dc:creator "Kiril Penev"@en ;
                  
                  skos:definition "Type of treatment activities performed on a cultural object during one treatment operation."@en .




###  Generated by the OWL API (version 3.5.0) http://owlapi.sourceforge.net

