@prefix : <http://www.semanticweb.org/owl/owlapi/turtle#> .
@prefix dc: <http://purl.org/dc/elements/1.1/> .
@prefix chc: <http://www.sirma.com/ontologies/2016/02/culturalHeritageConservation#> .
@prefix emf: <http://ittruse.ittbg.com/ontology/enterpriseManagementFramework#> .
@prefix nga: <http://www.sirma.com/ontologies/2016/02/culturalHeritageConservation/NGA#> .
@prefix owl: <http://www.w3.org/2002/07/owl#> .
@prefix rdf: <http://www.w3.org/1999/02/22-rdf-syntax-ns#> .
@prefix sec: <http://www.sirma.com/ontologies/2014/11/security#> .
@prefix xml: <http://www.w3.org/XML/1998/namespace> .
@prefix xsd: <http://www.w3.org/2001/XMLSchema#> .
@prefix ptop: <http://www.ontotext.com/proton/protontop#> .
@prefix rdfs: <http://www.w3.org/2000/01/rdf-schema#> .
@prefix skos: <http://www.w3.org/2004/02/skos/core#> .
@prefix dcterms: <http://purl.org/dc/terms/> .
@base <http://www.sirma.com/ontologies/2016/02/culturalHeritageConservation/NGA> .

<http://www.sirma.com/ontologies/2016/02/culturalHeritageConservation/NGA> rdf:type owl:Ontology ;
                                                                           
                                                                           rdfs:label "Extension of Cultural Heritage Conservation Ontology Model for NGA"@en ;
                                                                           
                                                                           owl:versionInfo "0.1"@en ;
                                                                           
                                                                           dc:subject "Extension of Cultural Heritage Conservation Ontology Model for NGA"@en ;
                                                                           
                                                                           dc:creator "Lidiya Dimitrova"@en ;
                                                                           
                                                                           rdfs:comment "NGA Extension of Cultural Heritage Conservation Ontology Model for Conservation Space project"@en ;
                                                                           
                                                                           dc:rights "What rights?"@en ;
                                                                           
                                                                           owl:imports <http://www.sirma.com/ontologies/2016/02/culturalHeritageConservation> .


#################################################################
#
#    Object Properties
#
#################################################################


###  http://www.sirma.com/ontologies/2016/02/culturalHeritageConservation/NGA#associatedWith

nga:associatedWith rdf:type owl:ObjectProperty ,
                            owl:SymmetricProperty ;
                   
                   rdfs:label "is associated with"@en ;
                   
                   emf:isSearchable "true"^^xsd:boolean ;
                   
                   dc:creator "Lidiya Dimitrova" ;
                   
                   emf:auditEvent "+addAssociatedWith|-removeAssociatedWith|changeAssociatedWith" ;
                   
                   skos:definition "Indicates the cultural object is associated with anathor cultural object."@en ;
                   
                   rdfs:range chc:CulturalObject ;
                   
                   rdfs:domain chc:CulturalObject .





#################################################################
#
#    Data properties
#
#################################################################


###  http://www.sirma.com/ontologies/2016/02/culturalHeritageConservation/NGA#accessionNumber

nga:accessionNumber rdf:type owl:DatatypeProperty ;
                    
                    rdfs:label "Accession Number"@en ;
                    
                    rdfs:comment "" ;
                    
                    dc:creator "Kiril Penev"@en ;
                    
                    skos:definition "Unique institutional ID. Can be coded to be human readable and to express, for example, year/lot/number if acquisition or shelf location."@en ;
                    
                    rdfs:domain chc:CulturalObject ;
                    
                    rdfs:range xsd:string .



###  http://www.sirma.com/ontologies/2016/02/culturalHeritageConservation/NGA#activityPhase

nga:activityPhase rdf:type owl:DatatypeProperty ;
                  
                  rdfs:label "Examination/Treatment Phase"@en ;
                  
                  dc:creator "Lidiya Dimitrova"@en ;
                  
                  skos:definition "The stage of the treatment/examination."@en ;
                  
                  rdfs:domain emf:Image ;
                  
                  rdfs:range xsd:string .



###  http://www.sirma.com/ontologies/2016/02/culturalHeritageConservation/NGA#analysisDate

nga:analysisDate rdf:type owl:DatatypeProperty ;
                 
                 rdfs:label "Date of analysis"@en ;
                 
                 dc:creator "Lidiya Dimitrova" ;
                 
                 skos:definition "The date of any analysis made on the sample."@en ;
                 
                 rdfs:domain emf:Document ;
                 
                 rdfs:range xsd:dateTime .



###  http://www.sirma.com/ontologies/2016/02/culturalHeritageConservation/NGA#analysisSummary

nga:analysisSummary rdf:type owl:DatatypeProperty ;
                    
                    rdfs:label "Analysis Summary"@en ;
                    
                    dc:creator "Lidiya Dimitrova"@en ;
                    
                    skos:definition "Summary description of the what was found by the analysis on the sample."@en ;
                    
                    rdfs:domain emf:Document ;
                    
                    rdfs:range xsd:string .



###  http://www.sirma.com/ontologies/2016/02/culturalHeritageConservation/NGA#appliedMediaCondition

nga:appliedMediaCondition rdf:type owl:DatatypeProperty ;
                          
                          rdfs:label "Applied Media Condition"@en ;
                          
                          skos:definition "Condition of the media applied to a photograph."@en ;
                          
                          dc:creator "Lidiya Dimitrova"@en ;
                          
                          rdfs:domain ptop:Document ;
                          
                          rdfs:subPropertyOf chc:condition ;
                          
                          rdfs:range xsd:string .



###  http://www.sirma.com/ontologies/2016/02/culturalHeritageConservation/NGA#appliedMediaDescription

nga:appliedMediaDescription rdf:type owl:DatatypeProperty ;
                            
                            rdfs:label "Applied Media Description"@en ;
                            
                            skos:definition "Description of media applied to photograph or to surface coating (eg retouching or hand coloring)"@en ;
                            
                            dc:creator "Lidiya Dimitrova"@en ;
                            
                            rdfs:domain nga:Photograph ;
                            
                            rdfs:range xsd:string .



###  http://www.sirma.com/ontologies/2016/02/culturalHeritageConservation/NGA#artistInstructions

nga:artistInstructions rdf:type owl:DatatypeProperty ;
                       
                       rdfs:label "Artist Instructions"@en ;
                       
                       skos:definition "Artists description of how the work is to be displayed/installed."@en ;
                       
                       dc:creator "Lidiya Dimitrova"@en ;
                       
                       rdfs:domain nga:MediaArt ;
                       
                       rdfs:range xsd:string .



###  http://www.sirma.com/ontologies/2016/02/culturalHeritageConservation/NGA#artistNames

nga:artistNames rdf:type owl:DatatypeProperty ;
                
                rdfs:label "Artist(s)"@en ;
                
                skos:definition "An entity primarily responsible for creating an object."@en ;
                
                dc:creator "Lidiya Dimitrova"@en ;
                
                rdfs:domain chc:CulturalObject ;
                
                rdfs:range xsd:string .



###  http://www.sirma.com/ontologies/2016/02/culturalHeritageConservation/NGA#assetCreator

nga:assetCreator rdf:type owl:DatatypeProperty ;
                 
                 rdfs:label "Creator"@en ;
                 
                 dc:creator "Lidiya Dimitrova"@en ;
                 
                 skos:definition "Name of asset creator  (scanned images or derivative files not created by original photographer)."@en ;
                 
                 rdfs:domain emf:Image ;
                 
                 rdfs:range xsd:string .



###  http://www.sirma.com/ontologies/2016/02/culturalHeritageConservation/NGA#associatedMaterials

nga:associatedMaterials rdf:type owl:DatatypeProperty ;
                        
                        rdfs:label "Associated Materials"@en ;
                        
                        dc:creator "Lidiya Dimitrova"@en ;
                        
                        skos:definition "This would include materials provided by the artist that are used for installation/adjustment/repair of the work of art, but are not actually part of the work of art."@en ;
                        
                        rdfs:domain nga:MediaArt ;
                        
                        rdfs:range xsd:string .



###  http://www.sirma.com/ontologies/2016/02/culturalHeritageConservation/NGA#barCode

nga:barCode rdf:type owl:DatatypeProperty ;
            
            rdfs:label "Bar Code"@en ;
            
            dc:creator "Lidiya Dimitrova"@en ;
            
            skos:definition "Symbol representation of the barcode."@en ;
            
            rdfs:domain nga:Frame ;
            
            rdfs:range xsd:string .



###  http://www.sirma.com/ontologies/2016/02/culturalHeritageConservation/NGA#baseCondition

nga:baseCondition rdf:type owl:DatatypeProperty ;
                  
                  rdfs:label "Base Condition"@en ;
                  
                  skos:definition "Description of the condition of the base of the cultural object."@en ;
                  
                  dc:creator "Lidiya Dimitrova"@en ;
                  
                  rdfs:domain ptop:Document ;
                  
                  rdfs:subPropertyOf chc:condition ;
                  
                  rdfs:range xsd:string .



###  http://www.sirma.com/ontologies/2016/02/culturalHeritageConservation/NGA#baseDescription

nga:baseDescription rdf:type owl:DatatypeProperty ;
                    
                    rdfs:label "Base Description"@en ;
                    
                    skos:definition "Description of the base for the cultural object, normally on a statue or sculpture. The bottom support of anything; that on which a thing stands or rests."@en ;
                    
                    dc:creator "Lidiya Dimitrova"@en ;
                    
                    rdfs:domain chc:CulturalObject ;
                    
                    rdfs:range xsd:string .



###  http://www.sirma.com/ontologies/2016/02/culturalHeritageConservation/NGA#bibliography

nga:bibliography rdf:type owl:DatatypeProperty ;
                 
                 rdfs:label "Bibliography"@en ;
                 
                 skos:definition """A bibliography is a list of all of the sources used (whether referenced or not) in the process of researching. In general, a bibliography should include:
    · the authors' names
    · the titles of the works
    · the names and locations of the companies that published your copies of the sources
    · the dates your copies were published
    · the page numbers of your sources (if they are part of multi-source volumes)"""@en ;
                 
                 dc:creator "Lidiya Dimitrova"@en ;
                 
                 rdfs:domain chc:CulturalObject ;
                 
                 rdfs:range xsd:string .



###  http://www.sirma.com/ontologies/2016/02/culturalHeritageConservation/NGA#binderCondition

nga:binderCondition rdf:type owl:DatatypeProperty ;
                    
                    rdfs:label "Binder Condition"@en ;
                    
                    skos:definition "Description of the condition of the binder."@en ;
                    
                    dc:creator "Lidiya Dimitrova"@en ;
                    
                    rdfs:domain ptop:Document ;
                    
                    rdfs:subPropertyOf chc:condition ;
                    
                    rdfs:range xsd:string .



###  http://www.sirma.com/ontologies/2016/02/culturalHeritageConservation/NGA#binderMaterial

nga:binderMaterial rdf:type owl:DatatypeProperty ;
                   
                   rdfs:label "Binder Material"@en ;
                   
                   dc:creator "Lidiya Dimitrova" ;
                   
                   skos:definition "Description of any material that holds the light sensitive materials."@en ;
                   
                   rdfs:domain nga:Photograph ;
                   
                   rdfs:range xsd:string .



###  http://www.sirma.com/ontologies/2016/02/culturalHeritageConservation/NGA#bindingCovering

nga:bindingCovering rdf:type owl:DatatypeProperty ;
                    
                    rdfs:label "Covering, decoration/finishing"@en ;
                    
                    dc:creator "Lidiya Dimitrova" ;
                    
                    skos:definition "Description of stamping, labels, or decoration to the binding."@en ;
                    
                    rdfs:domain nga:BoundVolume ;
                    
                    rdfs:range xsd:string .



###  http://www.sirma.com/ontologies/2016/02/culturalHeritageConservation/NGA#bindingStyle

nga:bindingStyle rdf:type owl:DatatypeProperty ;
                 
                 rdfs:label "Binding Style"@en ;
                 
                 skos:definition "Description of the binding style, materials and construction."@en ;
                 
                 dc:creator "Lidiya Dimitrova" ;
                 
                 rdfs:domain nga:BoundVolume ;
                 
                 rdfs:range xsd:string .



###  http://www.sirma.com/ontologies/2016/02/culturalHeritageConservation/NGA#borrowerName

nga:borrowerName rdf:type owl:DatatypeProperty ;
                 
                 rdfs:label "Borrower"@en ;
                 
                 dc:creator "Lidiya Dimitrova" ;
                 
                 skos:definition "The Institution that has borrowed the Cultural Object (outgoing Loan)"@en ;
                 
                 rdfs:domain ptop:Event ;
                 
                 rdfs:range xsd:string .



###  http://www.sirma.com/ontologies/2016/02/culturalHeritageConservation/NGA#callNumber

nga:callNumber rdf:type owl:DatatypeProperty ;
               
               rdfs:label "Call Number"@en ;
               
               dc:creator "Lidiya Dimitrova"@en ;
               
               skos:definition "NGA Library number"@en ;
               
               rdfs:domain chc:CulturalObject ;
               
               rdfs:range xsd:string .



###  http://www.sirma.com/ontologies/2016/02/culturalHeritageConservation/NGA#captureDevice

nga:captureDevice rdf:type owl:DatatypeProperty ;
                  
                  rdfs:label "Creator"@en ;
                  
                  dc:creator "Lidiya Dimitrova"@en ;
                  
                  skos:definition "The name of the camera or scanner."@en ;
                  
                  rdfs:domain emf:Image ;
                  
                  rdfs:range xsd:string .



###  http://www.sirma.com/ontologies/2016/02/culturalHeritageConservation/NGA#caseCondition

nga:caseCondition rdf:type owl:DatatypeProperty ;
                  
                  rdfs:label "Case Condition"@en ;
                  
                  skos:definition "Description of the case condition."@en ;
                  
                  dc:creator "Lidiya Dimitrova"@en ;
                  
                  rdfs:domain ptop:Document ;
                  
                  rdfs:subPropertyOf chc:condition ;
                  
                  rdfs:range xsd:string .



###  http://www.sirma.com/ontologies/2016/02/culturalHeritageConservation/NGA#caseDescription

nga:caseDescription rdf:type owl:DatatypeProperty ;
                    
                    rdfs:label "Case Description"@en ;
                    
                    skos:definition "Description of case, including exterior, hinge, interior, and textile if applicable."@en ;
                    
                    dc:creator "Lidiya Dimitrova"@en ;
                    
                    rdfs:domain nga:Photograph ;
                    
                    rdfs:range xsd:string .



###  http://www.sirma.com/ontologies/2016/02/culturalHeritageConservation/NGA#catalogueRaisonneRef

nga:catalogueRaisonneRef rdf:type owl:DatatypeProperty ;
                         
                         rdfs:label "Catalogue Raisonne Number"@en ;
                         
                         skos:definition "A global number of  the art work that appears in Catalogue Raisonne."@en ;
                         
                         dc:creator "Lidiya Dimitrova"@en ;
                         
                         rdfs:domain chc:CulturalObject ;
                         
                         rdfs:range xsd:string .



###  http://www.sirma.com/ontologies/2016/02/culturalHeritageConservation/NGA#century

nga:century rdf:type owl:DatatypeProperty ;
            
            rdfs:label "Century"@en ;
            
            dc:creator "Lidiya Dimitrova" ;
            
            skos:definition "The art object century."@en ;
            
            rdfs:domain nga:Frame ;
            
            rdfs:range xsd:string .



###  http://www.sirma.com/ontologies/2016/02/culturalHeritageConservation/NGA#collation

nga:collation rdf:type owl:DatatypeProperty ;
              
              rdfs:label "Textblock, collation"@en ;
              
              skos:definition "Description of the printer's imposition and organization of the gatherings in a textblock, expressed in a shorthand formula"@en ;
              
              dc:creator "Lidiya DImitrova"@en ;
              
              rdfs:domain nga:BoundVolume ;
              
              rdfs:range xsd:string .



###  http://www.sirma.com/ontologies/2016/02/culturalHeritageConservation/NGA#collection

nga:collection rdf:type owl:DatatypeProperty ;
               
               rdfs:label "Collection"@en ;
               
               dc:creator "Lidiya Dimitrova"@en ;
               
               skos:definition "NGA library grouping."@en ;
               
               rdfs:domain chc:CulturalObject ;
               
               rdfs:range xsd:string .



###  http://www.sirma.com/ontologies/2016/02/culturalHeritageConservation/NGA#contactDate

nga:contactDate rdf:type owl:DatatypeProperty ;
                
                rdfs:label "Date of Contact"@en ;
                
                skos:definition "Date of Contact."@en ;
                
                dc:creator "Lidiya Dimitrova"@en ;
                
                rdfs:domain emf:Document ;
                
                rdfs:range xsd:dateTime .



###  http://www.sirma.com/ontologies/2016/02/culturalHeritageConservation/NGA#contactPerson

nga:contactPerson rdf:type owl:DatatypeProperty ;
                  
                  rdfs:label "Contact Person"@en ;
                  
                  skos:definition "Contact Person"@en ;
                  
                  dc:creator "Lidiya Dimitrova"@en ;
                  
                  rdfs:domain emf:Document ;
                  
                  rdfs:range xsd:string .



###  http://www.sirma.com/ontologies/2016/02/culturalHeritageConservation/NGA#countryName

nga:countryName rdf:type owl:DatatypeProperty ;
                
                rdfs:label "Country/Region"@en ;
                
                dc:creator "Lidiya Dimitrova" ;
                
                skos:definition "The country/region to which the art object is related."@en ;
                
                rdfs:domain nga:Frame ;
                
                rdfs:range xsd:string .



###  http://www.sirma.com/ontologies/2016/02/culturalHeritageConservation/NGA#creationDates

nga:creationDates rdf:type owl:DatatypeProperty ;
                  
                  rdfs:label "Create Date(s)"@en ;
                  
                  dc:creator "Lidiya Dimitrova" ;
                  
                  skos:definition "Start/end dates and qualifiers such as \"circa\", \"before\", etc. Can have historical records of former attributions of creation dates."@en ;
                  
                  rdfs:domain chc:CulturalObject ;
                  
                  rdfs:range xsd:string .



###  http://www.sirma.com/ontologies/2016/02/culturalHeritageConservation/NGA#creditLine

nga:creditLine rdf:type owl:DatatypeProperty ;
               
               rdfs:label "Credit Line/Collection"@en ;
               
               dc:creator "Lidiya Dimitrova" ;
               
               skos:definition "Public credit line for the object. "@en ;
               
               rdfs:domain chc:CulturalObject ;
               
               rdfs:range xsd:string .



###  http://www.sirma.com/ontologies/2016/02/culturalHeritageConservation/NGA#culturalObjectViewDescription

nga:culturalObjectViewDescription rdf:type owl:DatatypeProperty ;
                                  
                                  rdfs:label "View Description"@en ;
                                  
                                  dc:creator "Lidiya Dimitrova"@en ;
                                  
                                  skos:definition "The view of the cultural object."@en ;
                                  
                                  rdfs:domain emf:Image ;
                                  
                                  rdfs:range xsd:string .



###  http://www.sirma.com/ontologies/2016/02/culturalHeritageConservation/NGA#curatorialRemarks

nga:curatorialRemarks rdf:type owl:DatatypeProperty ;
                      
                      rdfs:label "Curatorial Remarks"@en ;
                      
                      dc:creator "Lidiya Dimitrova" ;
                      
                      skos:definition "Notes made by the curator."@en ;
                      
                      rdfs:domain chc:CulturalObject ;
                      
                      rdfs:range xsd:string .



###  http://www.sirma.com/ontologies/2016/02/culturalHeritageConservation/NGA#currentLocation

nga:currentLocation rdf:type owl:DatatypeProperty ;
                    
                    rdfs:label "Current Location"@en ;
                    
                    dc:creator "Lidiya Dimitrova" ;
                    
                    skos:definition "The location that the object is physically resides currently."@en ;
                    
                    rdfs:domain chc:CulturalObject ;
                    
                    rdfs:range xsd:string .



###  http://www.sirma.com/ontologies/2016/02/culturalHeritageConservation/NGA#design

nga:design rdf:type owl:DatatypeProperty ;
           
           rdfs:label "Design"@en ;
           
           skos:definition "Description of the art object design. The arrangement of the features as produced from following a plan."@en ;
           
           dc:creator "Lidiya Dimitrova"@en ;
           
           rdfs:domain chc:CulturalObject ;
           
           rdfs:range xsd:string .



###  http://www.sirma.com/ontologies/2016/02/culturalHeritageConservation/NGA#designatedOpening

nga:designatedOpening rdf:type owl:DatatypeProperty ;
                      
                      rdfs:label "Designated Opening"@en ;
                      
                      dc:creator "Lidiya Dimitrova"@en ;
                      
                      skos:definition "The page to be displayed on the exhibition."@en ;
                      
                      rdfs:range xsd:string .



###  http://www.sirma.com/ontologies/2016/02/culturalHeritageConservation/NGA#designatedOpeningCondition

nga:designatedOpeningCondition rdf:type owl:DatatypeProperty ;
                               
                               rdfs:label "Designated Opening Condition"@en ;
                               
                               skos:definition "Description of the case designated opening condition."@en ;
                               
                               dc:creator "Lidiya Dimitrova"@en ;
                               
                               rdfs:domain emf:Document ;
                               
                               rdfs:subPropertyOf chc:condition ;
                               
                               rdfs:range xsd:string .



###  http://www.sirma.com/ontologies/2016/02/culturalHeritageConservation/NGA#displayedPages

nga:displayedPages rdf:type owl:DatatypeProperty ;
                   
                   rdfs:label "Displayed Pages"@en ;
                   
                   skos:definition "Identification of pages from Bound Volume that will be displayed in case the page does not have accession by itself."@en ;
                   
                   dc:creator "Lidiya Dimitrova"@en ;
                   
                   rdfs:range xsd:string .



###  http://www.sirma.com/ontologies/2016/02/culturalHeritageConservation/NGA#distinguishingMarks

nga:distinguishingMarks rdf:type owl:DatatypeProperty ;
                        
                        rdfs:label "Distinguishing Marks"@en ;
                        
                        skos:definition "Indication of distinguishing marks that have been applied to an object, including manufacturer's marks and labels, publisher's and printer's blind stamps."@en ;
                        
                        dc:creator "Lidiya Dimitrova"@en ;
                        
                        rdfs:domain chc:CulturalObject ;
                        
                        rdfs:range xsd:string .



###  http://www.sirma.com/ontologies/2016/02/culturalHeritageConservation/NGA#donorName

nga:donorName rdf:type owl:DatatypeProperty ;
              
              rdfs:label "Donor Name"@en ;
              
              dc:creator "Lidiya Dimitrova"@en ;
              
              skos:definition "Name of the donor of the frame."@en ;
              
              rdfs:domain nga:Frame ;
              
              rdfs:range xsd:string .



###  http://www.sirma.com/ontologies/2016/02/culturalHeritageConservation/NGA#edition

nga:edition rdf:type owl:DatatypeProperty ;
            
            rdfs:label "Edition"@en ;
            
            dc:creator "Lidiya Dimitrova" ;
            
            skos:definition "Number of the volumn or set, usually includes year."@en ;
            
            rdfs:domain chc:CulturalObject ;
            
            rdfs:range xsd:string .



###  http://www.sirma.com/ontologies/2016/02/culturalHeritageConservation/NGA#environmentalRequirements

nga:environmentalRequirements rdf:type owl:DatatypeProperty ;
                              
                              rdfs:label "Environmental Notes"@en ;
                              
                              skos:definition "Description of any special environmental notes that the cultural object may require."@en ;
                              
                              dc:creator "Lidiya Dimitrova"@en ;
                              
                              rdfs:domain chc:CulturalObject ;
                              
                              rdfs:range xsd:string .



###  http://www.sirma.com/ontologies/2016/02/culturalHeritageConservation/NGA#essentialComponents

nga:essentialComponents rdf:type owl:DatatypeProperty ;
                        
                        rdfs:label "Essential Components"@en ;
                        
                        dc:creator "Lidiya Dimitrova"@en ;
                        
                        skos:definition "The parts of the artwork that artist indicates cannot be changed or replaced"@en ;
                        
                        rdfs:domain chc:CulturalObject ;
                        
                        rdfs:range xsd:string .



###  http://www.sirma.com/ontologies/2016/02/culturalHeritageConservation/NGA#estimatedExpenses

nga:estimatedExpenses rdf:type owl:DatatypeProperty ;
                      
                      rdfs:label "Estimated Expenses"@en ;
                      
                      skos:definition "Estimated expenses for the project"@en ;
                      
                      dc:creator "Lidiya Dimitrova"@en ;
                      
                      rdfs:range xsd:string .



###  http://www.sirma.com/ontologies/2016/02/culturalHeritageConservation/NGA#exhibitionId

nga:exhibitionId rdf:type owl:DatatypeProperty ;
                 
                 rdfs:label "Exhibition ID"@en ;
                 
                 dc:creator "Lidiya Dimitrova"@en ;
                 
                 skos:definition "The tracking number to track each object with in an Incoming or outgoing Loans for an Exhibition."@en ;
                 
                 rdfs:range xsd:string .



###  http://www.sirma.com/ontologies/2016/02/culturalHeritageConservation/NGA#expectedOutcome

nga:expectedOutcome rdf:type owl:DatatypeProperty ;
                    
                    rdfs:label "Expected Outcome"@en ;
                    
                    skos:definition "Expected outcome of a project"@en ;
                    
                    dc:creator "Lidiya Dimitrova"@en ;
                    
                    rdfs:range xsd:string .



###  http://www.sirma.com/ontologies/2016/02/culturalHeritageConservation/NGA#fabricationMethod

nga:fabricationMethod rdf:type owl:DatatypeProperty ;
                      
                      rdfs:label "Fabrication Description"@en ;
                      
                      skos:definition "Description of the fabrication method of the art object."@en ;
                      
                      dc:creator "Lidiya Dimitrova"@en ;
                      
                      rdfs:domain chc:CulturalObject ;
                      
                      rdfs:range xsd:string .



###  http://www.sirma.com/ontologies/2016/02/culturalHeritageConservation/NGA#frameCondition

nga:frameCondition rdf:type owl:DatatypeProperty ;
                   
                   rdfs:label "Frame Conditionn"@en ;
                   
                   skos:definition "Description of condition of the frame."@en ;
                   
                   dc:creator "Lidiya Dimitrova"@en ;
                   
                   rdfs:subPropertyOf chc:condition ;
                   
                   rdfs:range xsd:string .



###  http://www.sirma.com/ontologies/2016/02/culturalHeritageConservation/NGA#frameDescription

nga:frameDescription rdf:type owl:DatatypeProperty ;
                     
                     rdfs:label "Frame Description"@en ;
                     
                     skos:definition "Description of the framing overall process and material, the frame itself, if part of the original art object or if the object is permanently framed in storage. Include glazing, framing package and backing."@en ;
                     
                     dc:creator "Lidiya Dimitrova"@en ;
                     
                     rdfs:domain chc:CulturalObject ;
                     
                     rdfs:range xsd:string .



###  http://www.sirma.com/ontologies/2016/02/culturalHeritageConservation/NGA#frameInnerDimensions

nga:frameInnerDimensions rdf:type owl:DatatypeProperty ;
                         
                         rdfs:label "Inner Dimensions"@en ;
                         
                         skos:definition "Inside dimension of the Frame (height and width)"@en ;
                         
                         dc:creator "Lidiya Dimitrova"@en ;
                         
                         rdfs:domain nga:Frame ;
                         
                         rdfs:range xsd:string .



###  http://www.sirma.com/ontologies/2016/02/culturalHeritageConservation/NGA#frameMoldingWidth

nga:frameMoldingWidth rdf:type owl:DatatypeProperty ;
                      
                      rdfs:label "Molding"@en ;
                      
                      dc:creator "Lidiya Dimitrova"@en ;
                      
                      skos:definition "The measurement from the site edge to the outer edge of the frame."@en ;
                      
                      rdfs:domain nga:Frame ;
                      
                      rdfs:range xsd:string .



###  http://www.sirma.com/ontologies/2016/02/culturalHeritageConservation/NGA#frameNotes

nga:frameNotes rdf:type owl:DatatypeProperty ;
               
               rdfs:label "Frame Notes"@en ;
               
               skos:definition "Additinal notes on the frame condition."@en ;
               
               dc:creator "Lidiya Dimitrova"@en ;
               
               rdfs:domain nga:Frame ;
               
               rdfs:range xsd:string .



###  http://www.sirma.com/ontologies/2016/02/culturalHeritageConservation/NGA#frameNumber

nga:frameNumber rdf:type owl:DatatypeProperty ;
                
                rdfs:label "Frame Number"@en ;
                
                dc:creator "Lidiya Dimitrova"@en ;
                
                skos:definition "Unique institutional Frame ID."@en ;
                
                rdfs:domain nga:Frame ;
                
                rdfs:range xsd:string .



###  http://www.sirma.com/ontologies/2016/02/culturalHeritageConservation/NGA#frameOutsideDimensions

nga:frameOutsideDimensions rdf:type owl:DatatypeProperty ;
                           
                           rdfs:label "Outside Dimensions"@en ;
                           
                           dc:creator "Lidiya Dimitrova"@en ;
                           
                           skos:definition "Outer dimension of the Frame (height and width)"@en ;
                           
                           rdfs:domain nga:Frame ;
                           
                           rdfs:range xsd:string .



###  http://www.sirma.com/ontologies/2016/02/culturalHeritageConservation/NGA#frameQuantity

nga:frameQuantity rdf:type owl:DatatypeProperty ;
                  
                  rdfs:label "Quantity"@en ;
                  
                  dc:creator "Lidiya Dimitrova"@en ;
                  
                  skos:definition "The count of the same type of the frame that are held in inventory."@en ;
                  
                  rdfs:domain nga:Frame ;
                  
                  rdfs:range xsd:string .



###  http://www.sirma.com/ontologies/2016/02/culturalHeritageConservation/NGA#frameRabbetDepth

nga:frameRabbetDepth rdf:type owl:DatatypeProperty ;
                     
                     rdfs:label "Rabbet Depth"@en ;
                     
                     dc:creator "Lidiya Dimitrova"@en ;
                     
                     skos:definition "Outer dimension of the Frame (height and width)"@en ;
                     
                     rdfs:domain nga:Frame ;
                     
                     rdfs:range xsd:string .



###  http://www.sirma.com/ontologies/2016/02/culturalHeritageConservation/NGA#frameShape

nga:frameShape rdf:type owl:DatatypeProperty ;
               
               rdfs:label "Shape"@en ;
               
               skos:definition "Description of the frame shape."@en ;
               
               dc:creator "Lidiya Dimitrova"@en ;
               
               rdfs:domain nga:Frame ;
               
               rdfs:range xsd:string .



###  http://www.sirma.com/ontologies/2016/02/culturalHeritageConservation/NGA#frameSiteSize

nga:frameSiteSize rdf:type owl:DatatypeProperty ;
                  
                  rdfs:label "Site Size"@en ;
                  
                  dc:creator "Lidiya Dimitrova"@en ;
                  
                  skos:definition "The size of the opening from the front of the frame.  "@en ;
                  
                  rdfs:domain nga:Frame ;
                  
                  rdfs:range xsd:string .



###  http://www.sirma.com/ontologies/2016/02/culturalHeritageConservation/NGA#framingPackage

nga:framingPackage rdf:type owl:DatatypeProperty ;
                   
                   rdfs:label "Framing Package"@en ;
                   
                   skos:definition "Description of framing package components put together by the institution including frame, glazing, and backing"@en ;
                   
                   dc:creator "Lidiya Dimitrova"@en ;
                   
                   rdfs:domain chc:CulturalObject ;
                   
                   rdfs:range xsd:string .



###  http://www.sirma.com/ontologies/2016/02/culturalHeritageConservation/NGA#framingPackageCondition

nga:framingPackageCondition rdf:type owl:DatatypeProperty ;
                            
                            rdfs:label "Framing Package Condition"@en ;
                            
                            skos:definition "Description of the condition of the cultural object framing package."@en ;
                            
                            dc:creator "Lidiya Dimitrova"@en ;
                            
                            rdfs:domain ptop:Document ;
                            
                            rdfs:subPropertyOf chc:condition ;
                            
                            rdfs:range xsd:string .



###  http://www.sirma.com/ontologies/2016/02/culturalHeritageConservation/NGA#glazeDescription

nga:glazeDescription rdf:type owl:DatatypeProperty ;
                     
                     rdfs:label "Glaze"@en ;
                     
                     dc:creator "Lidiya Dimitrova"@en ;
                     
                     skos:definition "Technical description of the glazing or any unusual glazing requirement such as Optium for a friable drawing. The glaze is a translucent colored material, usually a varnish, used as a painting technique."@en ;
                     
                     rdfs:domain chc:CulturalObject ;
                     
                     rdfs:range xsd:string .



###  http://www.sirma.com/ontologies/2016/02/culturalHeritageConservation/NGA#handlingRequirements

nga:handlingRequirements rdf:type owl:DatatypeProperty ;
                         
                         rdfs:label "Humidity Requirements "@en ;
                         
                         skos:definition "Description of any special handling that the cultural object may require."@en ;
                         
                         dc:creator "Lidiya Dimitrova"@en ;
                         
                         rdfs:domain chc:CulturalObject ;
                         
                         rdfs:range xsd:string .



###  http://www.sirma.com/ontologies/2016/02/culturalHeritageConservation/NGA#homeLocation

nga:homeLocation rdf:type owl:DatatypeProperty ;
                 
                 rdfs:label "Home Location"@en ;
                 
                 skos:definition "A gallery, storage location or  place within the organizatio where the cultural object normally is."@en ;
                 
                 dc:creator "Lidiya Dimitrova"@en ;
                 
                 rdfs:domain chc:CulturalObject ;
                 
                 rdfs:range xsd:string .



###  http://www.sirma.com/ontologies/2016/02/culturalHeritageConservation/NGA#housingCondition

nga:housingCondition rdf:type owl:DatatypeProperty ;
                     
                     rdfs:label "Housing Condition"@en ;
                     
                     skos:definition "Description of the condition of the housing of the cultural object."@en ;
                     
                     dc:creator "Lidiya Dimitrova"@en ;
                     
                     rdfs:domain ptop:Document ;
                     
                     rdfs:subPropertyOf chc:condition ;
                     
                     rdfs:range xsd:string .



###  http://www.sirma.com/ontologies/2016/02/culturalHeritageConservation/NGA#housingDescription

nga:housingDescription rdf:type owl:DatatypeProperty ;
                       
                       rdfs:label "Housing Description"@en ;
                       
                       skos:definition "Description of the permanent/important/original housing, such as box, slip case, original mats or folders, its materials and construction."@en ;
                       
                       dc:creator "Lidiya Dimitrova"@en ;
                       
                       rdfs:domain chc:CulturalObject ;
                       
                       rdfs:range xsd:string .



###  http://www.sirma.com/ontologies/2016/02/culturalHeritageConservation/NGA#imageCapturedSource

nga:imageCapturedSource rdf:type owl:DatatypeProperty ;
                        
                        rdfs:label "Captured Source"@en ;
                        
                        dc:creator "Lidiya Dimitrova"@en ;
                        
                        skos:definition "The source of the image. Information related to the origination of the image (where it came from)."@en ;
                        
                        rdfs:domain emf:Image ;
                        
                        rdfs:range xsd:string .



###  http://www.sirma.com/ontologies/2016/02/culturalHeritageConservation/NGA#imageLayerCondition

nga:imageLayerCondition rdf:type owl:DatatypeProperty ;
                        
                        rdfs:label "Image Layer Condition"@en ;
                        
                        skos:definition "Description of the condition of the image layer."@en ;
                        
                        dc:creator "Lidiya Dimitrova"@en ;
                        
                        rdfs:domain emf:Document ;
                        
                        rdfs:subPropertyOf chc:condition ;
                        
                        rdfs:range xsd:string .



###  http://www.sirma.com/ontologies/2016/02/culturalHeritageConservation/NGA#imageLayerDescription

nga:imageLayerDescription rdf:type owl:DatatypeProperty ;
                          
                          rdfs:label "Image Layer Description"@en ;
                          
                          skos:definition "Description of the final image layer of photograph."@en ;
                          
                          dc:creator "Lidiya Dimitrova"@en ;
                          
                          rdfs:domain nga:Photograph ;
                          
                          rdfs:range xsd:string .



###  http://www.sirma.com/ontologies/2016/02/culturalHeritageConservation/NGA#imageOriginalIdentifier

nga:imageOriginalIdentifier rdf:type owl:DatatypeProperty ;
                            
                            rdfs:label "Original Identifier"@en ;
                            
                            dc:creator "Lidiya Dimitrova"@en ;
                            
                            skos:definition "Name of the file from which a user creates the derivative. .DNG, raw, master ."@en ;
                            
                            rdfs:domain emf:Image ;
                            
                            rdfs:range xsd:string .



###  http://www.sirma.com/ontologies/2016/02/culturalHeritageConservation/NGA#imageProductDate

nga:imageProductDate rdf:type owl:DatatypeProperty ;
                     
                     rdfs:label "Product Date"@en ;
                     
                     dc:creator "Lidiya Dimitrova"@en ;
                     
                     skos:definition "The date that the image was produced. "@en ;
                     
                     rdfs:domain emf:Image ;
                     
                     rdfs:range xsd:dateTime .



###  http://www.sirma.com/ontologies/2016/02/culturalHeritageConservation/NGA#imageProductType

nga:imageProductType rdf:type owl:DatatypeProperty ;
                     
                     rdfs:label "Product Type"@en ;
                     
                     dc:creator "Lidiya Dimitrova"@en ;
                     
                     skos:definition "The product type defines if the image is original raw data or product derivative"@en ;
                     
                     rdfs:domain emf:Image ;
                     
                     rdfs:range xsd:string .



###  http://www.sirma.com/ontologies/2016/02/culturalHeritageConservation/NGA#imageSourceInstitution

nga:imageSourceInstitution rdf:type owl:DatatypeProperty ;
                           
                           rdfs:label "Source Institution"@en ;
                           
                           dc:creator "Lidiya Dimitrova"@en ;
                           
                           skos:definition "TSource-Institution of the image, department."@en ;
                           
                           rdfs:domain emf:Image ;
                           
                           rdfs:range xsd:string .



###  http://www.sirma.com/ontologies/2016/02/culturalHeritageConservation/NGA#imageSourceType

nga:imageSourceType rdf:type owl:DatatypeProperty ;
                    
                    rdfs:label "Source Type"@en ;
                    
                    dc:creator "Lidiya Dimitrova"@en ;
                    
                    skos:definition "The format of the source image."@en ;
                    
                    rdfs:domain emf:Image ;
                    
                    rdfs:range xsd:string .



###  http://www.sirma.com/ontologies/2016/02/culturalHeritageConservation/NGA#incomingLoanNumber

nga:incomingLoanNumber rdf:type owl:DatatypeProperty ;
                       
                       rdfs:label "In Coming Loan Number"@en ;
                       
                       dc:creator "Lidiya Dimitrova"@en ;
                       
                       skos:definition "Unique  number that is assigned to a Loan for an Exhibition inside of the organization."@en ;
                       
                       rdfs:range xsd:string .



###  http://www.sirma.com/ontologies/2016/02/culturalHeritageConservation/NGA#inscriptions

nga:inscriptions rdf:type owl:DatatypeProperty ;
                 
                 rdfs:label "Inscription(s)"@en ;
                 
                 skos:definition "Description of any writing or printing on the object's obverse or reverse. Artist signature, dealer marks, inventory codes, etc."@en ;
                 
                 dc:creator "Lidiya Dimitrova" ;
                 
                 rdfs:domain chc:CulturalObject ;
                 
                 rdfs:range xsd:string .



###  http://www.sirma.com/ontologies/2016/02/culturalHeritageConservation/NGA#installationRequirements

nga:installationRequirements rdf:type owl:DatatypeProperty ;
                             
                             rdfs:label "Installation Requirements" ;
                             
                             dc:creator "Lidiya Dimitrova" ;
                             
                             skos:definition "Any special Installation Instruction that the cultural object may require" ;
                             
                             rdfs:domain chc:CulturalObject ;
                             
                             rdfs:range xsd:string .



###  http://www.sirma.com/ontologies/2016/02/culturalHeritageConservation/NGA#laminateCondition

nga:laminateCondition rdf:type owl:DatatypeProperty ;
                      
                      rdfs:label "Laminate Condition"@en ;
                      
                      skos:definition "Description of the laminate condition."@en ;
                      
                      dc:creator "Lidiya Dimitrova"@en ;
                      
                      rdfs:domain emf:Document ;
                      
                      rdfs:subPropertyOf chc:condition ;
                      
                      rdfs:range xsd:string .



###  http://www.sirma.com/ontologies/2016/02/culturalHeritageConservation/NGA#laminateDescription

nga:laminateDescription rdf:type owl:DatatypeProperty ;
                        
                        rdfs:label "Laminate Description"@en ;
                        
                        skos:definition "Description of glazing, face mounting, or laminate (eg face mounted photographs, plastic laminate, ambrotype, integral frame)."@en ;
                        
                        dc:creator "Lidiya Dimitrova"@en ;
                        
                        rdfs:domain nga:Photograph ;
                        
                        rdfs:range xsd:string .



###  http://www.sirma.com/ontologies/2016/02/culturalHeritageConservation/NGA#lenderName

nga:lenderName rdf:type owl:DatatypeProperty ;
               
               rdfs:label "Lender"@en ;
               
               dc:creator "Lidiya Dimitrova" ;
               
               skos:definition "The institution that has lend the Cultural Object for the Exhibition."@en ;
               
               rdfs:range xsd:string .



###  http://www.sirma.com/ontologies/2016/02/culturalHeritageConservation/NGA#lightType

nga:lightType rdf:type owl:DatatypeProperty ;
              
              rdfs:label "Light Type"@en ;
              
              dc:creator "Lidiya Dimitrova"@en ;
              
              skos:definition "The type of light used for the photograph to be taken."@en ;
              
              rdfs:domain emf:Image ;
              
              rdfs:range xsd:string .



###  http://www.sirma.com/ontologies/2016/02/culturalHeritageConservation/NGA#manipulateType

nga:manipulateType rdf:type owl:DatatypeProperty ;
                   
                   rdfs:label "Manipulate Type"@en ;
                   
                   dc:creator "Lidiya Dimitrova"@en ;
                   
                   skos:definition "The manipulate type of the image e.g raw, histogram, color."@en ;
                   
                   rdfs:domain emf:Image ;
                   
                   rdfs:range xsd:string .



###  http://www.sirma.com/ontologies/2016/02/culturalHeritageConservation/NGA#manufactureMethod

nga:manufactureMethod rdf:type owl:DatatypeProperty ;
                      
                      rdfs:label "Method Of Manufacture"@en ;
                      
                      dc:creator "Lidiya Dimitrova"@en ;
                      
                      skos:definition "Specific details of how an object is made based on examination"@en ;
                      
                      rdfs:domain chc:CulturalObject ;
                      
                      rdfs:range xsd:string .



###  http://www.sirma.com/ontologies/2016/02/culturalHeritageConservation/NGA#manufacturerName

nga:manufacturerName rdf:type owl:DatatypeProperty ;
                     
                     rdfs:label "Manufacturer"@en ;
                     
                     dc:creator "Lidiya Dimitrova"@en ;
                     
                     skos:definition "The name of the product manufacturer"@en ;
                     
                     rdfs:range xsd:string .



###  http://www.sirma.com/ontologies/2016/02/culturalHeritageConservation/NGA#matAttachmentCondition

nga:matAttachmentCondition rdf:type owl:DatatypeProperty ;
                           
                           rdfs:label "Attachment Condition"@en ;
                           
                           skos:definition "Description of the condition of the cultural object attachment to the mat."@en ;
                           
                           dc:creator "Lidiya Dimitrova"@en ;
                           
                           rdfs:domain emf:Document ;
                           
                           rdfs:subPropertyOf chc:condition ;
                           
                           rdfs:range xsd:string .



###  http://www.sirma.com/ontologies/2016/02/culturalHeritageConservation/NGA#matAttachmentDescription

nga:matAttachmentDescription rdf:type owl:DatatypeProperty ;
                             
                             rdfs:label "Attachment Description"@en ;
                             
                             skos:definition "Description of how  the object is attached to the mat. (attachment method)"@en ;
                             
                             dc:creator "Lidiya Dimitrova"@en ;
                             
                             rdfs:domain chc:CulturalObject ;
                             
                             rdfs:range xsd:string .



###  http://www.sirma.com/ontologies/2016/02/culturalHeritageConservation/NGA#matCondition

nga:matCondition rdf:type owl:DatatypeProperty ;
                 
                 rdfs:label "Mat Condition"@en ;
                 
                 skos:definition "Description of the mat condition."@en ;
                 
                 dc:creator "Lidiya Dimitrova"@en ;
                 
                 rdfs:domain emf:Document ;
                 
                 rdfs:subPropertyOf chc:condition ;
                 
                 rdfs:range xsd:string .



###  http://www.sirma.com/ontologies/2016/02/culturalHeritageConservation/NGA#matDescription

nga:matDescription rdf:type owl:DatatypeProperty ;
                   
                   rdfs:label "Attachment Description"@en ;
                   
                   skos:definition "Description of how  the object is attached to the mat. (attachment method)"@en ;
                   
                   dc:creator "Lidiya Dimitrova"@en ;
                   
                   rdfs:domain chc:CulturalObject ;
                   
                   rdfs:range xsd:string .



###  http://www.sirma.com/ontologies/2016/02/culturalHeritageConservation/NGA#materialType

nga:materialType rdf:type owl:DatatypeProperty ;
                 
                 rdfs:label "Material type"@en ;
                 
                 skos:definition "Description of the material type."@en ;
                 
                 dc:creator "Lidiya Dimitrova"@en ;
                 
                 rdfs:range xsd:string .



###  http://www.sirma.com/ontologies/2016/02/culturalHeritageConservation/NGA#mediaCondition

nga:mediaCondition rdf:type owl:DatatypeProperty ;
                   
                   rdfs:label "Media Condition"@en ;
                   
                   skos:definition "Description of the condition of the media  such as media flaking, cracking, loss media abrasion, scratches, burnishing, media fading, media friable."@en ;
                   
                   dc:creator "Lidiya Dimitrova"@en ;
                   
                   rdfs:domain emf:Document ;
                   
                   rdfs:subPropertyOf chc:condition ;
                   
                   rdfs:range xsd:string .



###  http://www.sirma.com/ontologies/2016/02/culturalHeritageConservation/NGA#mediaDescription

nga:mediaDescription rdf:type owl:DatatypeProperty ;
                     
                     rdfs:label "Media"@en ;
                     
                     skos:definition "Description of the media used for the cultural object."@en ;
                     
                     dc:creator "Lidiya Dimitrova"@en ;
                     
                     rdfs:domain chc:CulturalObject ;
                     
                     rdfs:range xsd:string .



###  http://www.sirma.com/ontologies/2016/02/culturalHeritageConservation/NGA#medium

nga:medium rdf:type owl:DatatypeProperty ;
           
           rdfs:label "Material/Medium (very general)"@en ;
           
           dc:creator "Lidiya Dimitrova"@en ;
           
           skos:definition "Medium description often used for public."@en ;
           
           rdfs:domain chc:CulturalObject ;
           
           rdfs:range xsd:string .



###  http://www.sirma.com/ontologies/2016/02/culturalHeritageConservation/NGA#mountCondition

nga:mountCondition rdf:type owl:DatatypeProperty ;
                   
                   rdfs:label "Mount Condition"@en ;
                   
                   skos:definition "Description of the condition of the mount of the cultural object."@en ;
                   
                   dc:creator "Lidiya Dimitrova"@en ;
                   
                   rdfs:domain emf:Document ;
                   
                   rdfs:subPropertyOf chc:condition ;
                   
                   rdfs:range xsd:string .



###  http://www.sirma.com/ontologies/2016/02/culturalHeritageConservation/NGA#mountDescription

nga:mountDescription rdf:type owl:DatatypeProperty ;
                     
                     rdfs:label "Mount Description"@en ;
                     
                     dc:creator "Lidiya Dimitrova"@en ;
                     
                     skos:definition "Text description of the mounting when Art objects is on display."@en ;
                     
                     rdfs:domain chc:CulturalObject ;
                     
                     rdfs:range xsd:string .



###  http://www.sirma.com/ontologies/2016/02/culturalHeritageConservation/NGA#objectDepartmentName

nga:objectDepartmentName rdf:type owl:DatatypeProperty ;
                         
                         rdfs:label "Object Department"@en ;
                         
                         dc:creator "Lidiya Dimitrova"@en ;
                         
                         skos:definition "The object department responsible for the curatorial management and displaying for exhibition but acquisition is done by Registrar office."@en ;
                         
                         rdfs:domain chc:CulturalObject ;
                         
                         rdfs:range xsd:string .



###  http://www.sirma.com/ontologies/2016/02/culturalHeritageConservation/NGA#outgoingLoanNumber

nga:outgoingLoanNumber rdf:type owl:DatatypeProperty ;
                       
                       rdfs:label "Outgoing Loan Number" ;
                       
                       dc:creator "Lidiya Dimitrova" ;
                       
                       skos:definition "Unique  number that is assigned to a Loan for an Exhibition Outside of the organization and can have one or more objects." ;
                       
                       rdfs:range xsd:string .



###  http://www.sirma.com/ontologies/2016/02/culturalHeritageConservation/NGA#overallConditionAppraisal

nga:overallConditionAppraisal rdf:type owl:DatatypeProperty ;
                              
                              rdfs:label "Overall condition appraisal"@en ;
                              
                              skos:definition "General description of the condition of the cultural object."@en ;
                              
                              dc:creator "Lidiya Dimitrova"@en ;
                              
                              rdfs:domain emf:Document ;
                              
                              rdfs:subPropertyOf chc:condition ;
                              
                              rdfs:range xsd:string .



###  http://www.sirma.com/ontologies/2016/02/culturalHeritageConservation/NGA#ownerNames

nga:ownerNames rdf:type owl:DatatypeProperty ;
               
               rdfs:label "Owner/Custodian"@en ;
               
               dc:creator "Lidiya Dimitrova"@en ;
               
               skos:definition "The owner (person or organization) of a cultural object. The cultural object is not always a museum's possession."@en ;
               
               rdfs:domain chc:CulturalObject ;
               
               rdfs:range xsd:string .



###  http://www.sirma.com/ontologies/2016/02/culturalHeritageConservation/NGA#packingRequirements

nga:packingRequirements rdf:type owl:DatatypeProperty ;
                        
                        rdfs:label "Packing Notes"@en ;
                        
                        skos:definition "Description of any special packing notes/instructions for movement or transport  for this cultural object."@en ;
                        
                        dc:creator "Lidiya Dimitrova"@en ;
                        
                        rdfs:domain chc:CulturalObject ;
                        
                        rdfs:range xsd:string .



###  http://www.sirma.com/ontologies/2016/02/culturalHeritageConservation/NGA#paintLayersCondition

nga:paintLayersCondition rdf:type owl:DatatypeProperty ;
                         
                         rdfs:label "Paint Layers Condition"@en ;
                         
                         skos:definition "Description of the paint layer or design condition."@en ;
                         
                         dc:creator "Lidiya Dimitrova"@en ;
                         
                         rdfs:domain emf:Document ;
                         
                         rdfs:subPropertyOf chc:condition ;
                         
                         rdfs:range xsd:string .



###  http://www.sirma.com/ontologies/2016/02/culturalHeritageConservation/NGA#paintLayersDescription

nga:paintLayersDescription rdf:type owl:DatatypeProperty ;
                           
                           rdfs:label "Paint Layers Description"@en ;
                           
                           dc:creator "Lidiya Dimitrova"@en ;
                           
                           skos:definition "Technical description of the paint layer or design construction."@en ;
                           
                           rdfs:domain chc:CulturalObject ;
                           
                           rdfs:range xsd:string .



###  http://www.sirma.com/ontologies/2016/02/culturalHeritageConservation/NGA#photographerName

nga:photographerName rdf:type owl:DatatypeProperty ;
                     
                     rdfs:label "Photographer"@en ;
                     
                     dc:creator "Lidiya Dimitrova"@en ;
                     
                     skos:definition "Name of the photographer"@en ;
                     
                     rdfs:domain emf:Image ;
                     
                     rdfs:range xsd:string .



###  http://www.sirma.com/ontologies/2016/02/culturalHeritageConservation/NGA#physicalDimensions

nga:physicalDimensions rdf:type owl:DatatypeProperty ;
                       
                       rdfs:label "Base Physical Dimensions"@en ;
                       
                       dc:creator "Kiril Penev"@en ;
                       
                       skos:definition "The physical attributes of the object without matte and/or frame. Both US and metric. Can be complex with multi-component or 3-dimensional objects. Includes weight and other measures of the physical attributes of objects and their components."@en ;
                       
                       rdfs:domain chc:CulturalObject ;
                       
                       rdfs:range xsd:string .



###  http://www.sirma.com/ontologies/2016/02/culturalHeritageConservation/NGA#physicalLocation

nga:physicalLocation rdf:type owl:DatatypeProperty ;
                     
                     rdfs:label "Physical Location"@en ;
                     
                     dc:creator "Lidiya Dimitrova"@en ;
                     
                     skos:definition "Physical location of the sample so that someone could lay their hands on such as drawer number."@en ;
                     
                     rdfs:domain chc:Sample ;
                     
                     rdfs:range xsd:string .



###  http://www.sirma.com/ontologies/2016/02/culturalHeritageConservation/NGA#portfolioTitle

nga:portfolioTitle rdf:type owl:DatatypeProperty ;
                   
                   rdfs:label "Portfolio/Series"@en ;
                   
                   dc:creator "Lidiya Dimitrova" ;
                   
                   skos:definition "Indication of a group of works of art created as a group."@en ;
                   
                   rdfs:domain chc:CulturalObject ;
                   
                   rdfs:range xsd:string .



###  http://www.sirma.com/ontologies/2016/02/culturalHeritageConservation/NGA#preserverCondition

nga:preserverCondition rdf:type owl:DatatypeProperty ;
                       
                       rdfs:label "Preserver Condition"@en ;
                       
                       skos:definition "Description of the preserver condition."@en ;
                       
                       dc:creator "Lidiya Dimitrova"@en ;
                       
                       rdfs:domain emf:Document ;
                       
                       rdfs:subPropertyOf chc:condition ;
                       
                       rdfs:range xsd:string .



###  http://www.sirma.com/ontologies/2016/02/culturalHeritageConservation/NGA#preserverDescription

nga:preserverDescription rdf:type owl:DatatypeProperty ;
                         
                         rdfs:label "Preserver Description"@en ;
                         
                         skos:definition "Description of preserver in a cased object."@en ;
                         
                         dc:creator "Lidiya Dimitrova"@en ;
                         
                         rdfs:domain nga:Photograph ;
                         
                         rdfs:range xsd:string .



###  http://www.sirma.com/ontologies/2016/02/culturalHeritageConservation/NGA#primingCondition

nga:primingCondition rdf:type owl:DatatypeProperty ;
                     
                     rdfs:label "Sizing and Ground Condition"@en ;
                     
                     skos:definition "Description of the sizing and ground condition."@en ;
                     
                     dc:creator "Lidiya Dimitrova"@en ;
                     
                     rdfs:domain emf:Document ;
                     
                     rdfs:subPropertyOf chc:condition ;
                     
                     rdfs:range xsd:string .



###  http://www.sirma.com/ontologies/2016/02/culturalHeritageConservation/NGA#primingDescription

nga:primingDescription rdf:type owl:DatatypeProperty ;
                       
                       rdfs:label "Sizing and Ground Description"@en ;
                       
                       skos:definition "Description of the sizes and/or grounds applied to the primary support."@en ;
                       
                       dc:creator "Lidiya Dimitrova" ;
                       
                       rdfs:domain chc:CulturalObject ;
                       
                       rdfs:range xsd:string .



###  http://www.sirma.com/ontologies/2016/02/culturalHeritageConservation/NGA#productDescription

nga:productDescription rdf:type owl:DatatypeProperty ;
                       
                       rdfs:label "Description of Product"@en ;
                       
                       skos:definition "Description of product for analysis."@en ;
                       
                       dc:creator "Lidiya Dimitrova"@en ;
                       
                       rdfs:range xsd:string .



###  http://www.sirma.com/ontologies/2016/02/culturalHeritageConservation/NGA#provenance

nga:provenance rdf:type owl:DatatypeProperty ;
               
               rdfs:label "Provenance"@en ;
               
               skos:definition "Historical ownership of an art object."@en ;
               
               dc:creator "Lidiya Dimitrova"@en ;
               
               rdfs:domain chc:CulturalObject ;
               
               rdfs:range xsd:string .



###  http://www.sirma.com/ontologies/2016/02/culturalHeritageConservation/NGA#publicationDate

nga:publicationDate rdf:type owl:DatatypeProperty ;
                    
                    rdfs:label "Publication Date"@en ;
                    
                    skos:definition "Date of publication of the cultural object."@en ;
                    
                    dc:creator "Lidiya Dimitrova"@en ;
                    
                    rdfs:domain chc:CulturalObject ;
                    
                    rdfs:range xsd:string .



###  http://www.sirma.com/ontologies/2016/02/culturalHeritageConservation/NGA#publicationPlace

nga:publicationPlace rdf:type owl:DatatypeProperty ;
                     
                     rdfs:label "Place of publication"@en ;
                     
                     dc:creator "Lidiya Dimitrova" ;
                     
                     skos:definition "Identifies the city of publication."@en ;
                     
                     rdfs:domain nga:BoundVolume ;
                     
                     rdfs:range xsd:string .



###  http://www.sirma.com/ontologies/2016/02/culturalHeritageConservation/NGA#reportDate

nga:reportDate rdf:type owl:DatatypeProperty ;
               
               rdfs:label "Date of the report"@en ;
               
               dc:creator "Lidiya Dimitrova" ;
               
               skos:definition "Defines the date of the report. "@en ;
               
               rdfs:domain ptop:Document ;
               
               rdfs:range xsd:dateTime .



###  http://www.sirma.com/ontologies/2016/02/culturalHeritageConservation/NGA#sampleCondition

nga:sampleCondition rdf:type owl:DatatypeProperty ;
                    
                    rdfs:label "Sample Condition"@en ;
                    
                    dc:creator "Lidiya Dimitrova" ;
                    
                    skos:definition "Condition of the sample."@en ;
                    
                    rdfs:domain emf:Document ;
                    
                    rdfs:subPropertyOf chc:condition ;
                    
                    rdfs:range xsd:string .



###  http://www.sirma.com/ontologies/2016/02/culturalHeritageConservation/NGA#sampleMaterialsIdentified

nga:sampleMaterialsIdentified rdf:type owl:DatatypeProperty ;
                              
                              rdfs:label "Materials  identified"@en ;
                              
                              dc:creator "Lidiya Dimitrova"@en ;
                              
                              skos:definition "Materials identified in the analysis of the sample: for example \"chrome yellow in linseed oil."@en ;
                              
                              rdfs:range xsd:string .



###  http://www.sirma.com/ontologies/2016/02/culturalHeritageConservation/NGA#sampleSite

nga:sampleSite rdf:type owl:DatatypeProperty ;
               
               rdfs:label "Sample Site"@en ;
               
               dc:creator "Lidiya Dimitrova" ;
               
               skos:definition "Location of the spot where the sample was taken: coordinates \"up\" and \"left\" or \"from right hand of the sitter\"."@en ;
               
               rdfs:domain chc:Sample ;
               
               rdfs:range xsd:string .



###  http://www.sirma.com/ontologies/2016/02/culturalHeritageConservation/NGA#samplingDate

nga:samplingDate rdf:type owl:DatatypeProperty ;
                 
                 rdfs:label "Date taken"@en ;
                 
                 dc:creator "Lidiya Dimitrova" ;
                 
                 skos:definition "Date on which the sample was taken."@en ;
                 
                 rdfs:domain chc:Sample ;
                 
                 rdfs:range xsd:dateTime .



###  http://www.sirma.com/ontologies/2016/02/culturalHeritageConservation/NGA#samplingDateRequested

nga:samplingDateRequested rdf:type owl:DatatypeProperty ;
                          
                          rdfs:label "Date Requested"@en ;
                          
                          dc:creator "Lidiya Dimitrova" ;
                          
                          skos:definition "The data on which sample analysis is requested"@en ;
                          
                          rdfs:range xsd:dateTime .



###  http://www.sirma.com/ontologies/2016/02/culturalHeritageConservation/NGA#samplingReason

nga:samplingReason rdf:type owl:DatatypeProperty ;
                   
                   rdfs:label "Reason for sampling"@en ;
                   
                   dc:creator "Lidiya Dimitrova" ;
                   
                   skos:definition "Reason for sampling/motivation for sampling"@en ;
                   
                   rdfs:range xsd:string .



###  http://www.sirma.com/ontologies/2016/02/culturalHeritageConservation/NGA#secondarySupportCondition

nga:secondarySupportCondition rdf:type owl:DatatypeProperty ;
                              
                              rdfs:label "Secondary Support Condition"@en ;
                              
                              skos:definition "Description of any secondary support (stretcher, lining canvas, etc). The secondary support is  second, newer than the original, support for the cultural object. "@en ;
                              
                              dc:creator "Lidiya Dimitrova"@en ;
                              
                              rdfs:domain emf:Document ;
                              
                              rdfs:subPropertyOf chc:condition ;
                              
                              rdfs:range xsd:string .



###  http://www.sirma.com/ontologies/2016/02/culturalHeritageConservation/NGA#secondarySupportDescription

nga:secondarySupportDescription rdf:type owl:DatatypeProperty ;
                                
                                rdfs:label "Secondary support"@en ;
                                
                                skos:definition "Description of any secondary support (stretcher, lining canvas, etc). The secondary support is  second, newer than the original, support for the cultural object.  The support can be: For photograph -  glued or attached layer or material for support. For drawing -  thick laid paper. For painting - stretcher, lining canvas, etc."@en ;
                                
                                dc:creator "Lidiya Dimitrova"@en ;
                                
                                rdfs:domain chc:CulturalObject ;
                                
                                rdfs:range xsd:string .



###  http://www.sirma.com/ontologies/2016/02/culturalHeritageConservation/NGA#spectralRange

nga:spectralRange rdf:type owl:DatatypeProperty ;
                  
                  rdfs:label "Spectral Range"@en ;
                  
                  dc:creator "Lidiya Dimitrova"@en ;
                  
                  skos:definition "The type of light used for the photograph to be taken."@en ;
                  
                  rdfs:domain emf:Image ;
                  
                  rdfs:range xsd:string .



###  http://www.sirma.com/ontologies/2016/02/culturalHeritageConservation/NGA#structureCondition

nga:structureCondition rdf:type owl:DatatypeProperty ;
                       
                       rdfs:label "Structural Condition"@en ;
                       
                       skos:definition "Description of the condition of the structure of the cultural object."@en ;
                       
                       dc:creator "Lidiya Dimitrova"@en ;
                       
                       rdfs:domain emf:Document ;
                       
                       rdfs:subPropertyOf chc:condition ;
                       
                       rdfs:range xsd:string .



###  http://www.sirma.com/ontologies/2016/02/culturalHeritageConservation/NGA#structureDescription

nga:structureDescription rdf:type owl:DatatypeProperty ;
                         
                         rdfs:label "Structure Description"@en ;
                         
                         skos:definition "Description of the structure of the cultural objects - material used and the relationship between them."@en ;
                         
                         dc:creator "Lidiya Dimitrova"@en ;
                         
                         rdfs:domain chc:CulturalObject ;
                         
                         rdfs:range xsd:string .



###  http://www.sirma.com/ontologies/2016/02/culturalHeritageConservation/NGA#style

nga:style rdf:type owl:DatatypeProperty ;
          
          rdfs:label "Style"@en ;
          
          skos:definition "A way of Painting, drawing, building, composing, etc. Characteristic of a particular period, place, person or movement."@en ;
          
          dc:creator "Lidiya Dimitrova"@en ;
          
          rdfs:domain nga:Frame ;
          
          rdfs:range xsd:string .



###  http://www.sirma.com/ontologies/2016/02/culturalHeritageConservation/NGA#subClassification

nga:subClassification rdf:type owl:DatatypeProperty ;
                      
                      rdfs:label "Sub-Classification"@en ;
                      
                      dc:creator "Lidiya Dimitrova"@en ;
                      
                      skos:definition "Object sub-classification."@en ;
                      
                      rdfs:range xsd:string .



###  http://www.sirma.com/ontologies/2016/02/culturalHeritageConservation/NGA#substrateCondition

nga:substrateCondition rdf:type owl:DatatypeProperty ;
                       
                       rdfs:label "Substrate Condition"@en ;
                       
                       skos:definition "Description of the cultural object substrate. For decorative art cultural object this is is a layer before the surface, for a photograph this is the primary or underlying material on which other materials, such as ink, coating, paint, or treatment, are applied"@en ;
                       
                       dc:creator "Lidiya Dimitrova"@en ;
                       
                       rdfs:domain emf:Document ;
                       
                       rdfs:subPropertyOf chc:condition ;
                       
                       rdfs:range xsd:string .



###  http://www.sirma.com/ontologies/2016/02/culturalHeritageConservation/NGA#substrateDescription

nga:substrateDescription rdf:type owl:DatatypeProperty ;
                         
                         rdfs:label "Substrate Description"@en ;
                         
                         skos:definition "Description of the cultural object substrate. For decorative art cultural object this is is a layer before the surface, for a photograph this is the primary or underlying material on which other materials, such as ink, coating, paint, or treatment, are applied"@en ;
                         
                         dc:creator "Lidiya Dimitrova"@en ;
                         
                         rdfs:domain chc:CulturalObject ;
                         
                         rdfs:range xsd:string .



###  http://www.sirma.com/ontologies/2016/02/culturalHeritageConservation/NGA#supportCondition

nga:supportCondition rdf:type owl:DatatypeProperty ;
                     
                     rdfs:label "Support Condition"@en ;
                     
                     skos:definition "Description of the condition of the paper support. Example: torn and delaminating  chine colle"@en ;
                     
                     dc:creator "Lidiya Dimitrova"@en ;
                     
                     rdfs:domain emf:Document ;
                     
                     rdfs:subPropertyOf chc:condition ;
                     
                     rdfs:range xsd:string .



###  http://www.sirma.com/ontologies/2016/02/culturalHeritageConservation/NGA#supportDescription

nga:supportDescription rdf:type owl:DatatypeProperty ;
                       
                       rdfs:label "Support Description"@en ;
                       
                       skos:definition "Description of the support.  For painting it can be the canvas, paper, etc. For photograph it is the primary or underlying material on which other materials, such as ink, binder, coating, paint, or treatment, are applied: Paper(negative), Iron(tin type),glass(clodian, ambrotype), Film, Copper(silver dagurreotype), Polo-ride"@en ;
                       
                       dc:creator "Lidiya Dimitrova"@en ;
                       
                       rdfs:domain chc:CulturalObject ;
                       
                       rdfs:range xsd:string .



###  http://www.sirma.com/ontologies/2016/02/culturalHeritageConservation/NGA#surfaceCoatingCondition

nga:surfaceCoatingCondition rdf:type owl:DatatypeProperty ;
                            
                            rdfs:label "Surface Coating Condition"@en ;
                            
                            skos:definition "Description of the surface coating condition."@en ;
                            
                            dc:creator "Lidiya Dimitrova"@en ;
                            
                            rdfs:domain emf:Document ;
                            
                            rdfs:subPropertyOf chc:condition ;
                            
                            rdfs:range xsd:string .



###  http://www.sirma.com/ontologies/2016/02/culturalHeritageConservation/NGA#surfaceCoatingMaterial

nga:surfaceCoatingMaterial rdf:type owl:DatatypeProperty ;
                           
                           rdfs:label "Surface Coating Description"@en ;
                           
                           skos:definition "Description of the surface coating material (such as natural resins, waxes, gelatin, albumen, or anti-halation layer for film)."@en ;
                           
                           dc:creator "Lidiya Dimitrova"@en ;
                           
                           rdfs:domain chc:CulturalObject ;
                           
                           rdfs:range xsd:string .



###  http://www.sirma.com/ontologies/2016/02/culturalHeritageConservation/NGA#surfaceCondition

nga:surfaceCondition rdf:type owl:DatatypeProperty ;
                     
                     rdfs:label "Surface Condition "@en ;
                     
                     skos:definition "Description of the condition of the surface of the cultural object."@en ;
                     
                     dc:creator "Lidiya DImitrova"@en ;
                     
                     rdfs:domain emf:Document ;
                     
                     rdfs:subPropertyOf chc:condition ;
                     
                     rdfs:range xsd:string .



###  http://www.sirma.com/ontologies/2016/02/culturalHeritageConservation/NGA#surfaceDescription

nga:surfaceDescription rdf:type owl:DatatypeProperty ;
                       
                       rdfs:label "Surface Description"@en ;
                       
                       skos:definition "Description of the surface of an art objects. For sculpture this is the outside part or uppermost layer of something (often used when describing its texture, form, or extent)."@en ;
                       
                       dc:creator "Lidiya DImitrova"@en ;
                       
                       rdfs:domain chc:CulturalObject ;
                       
                       rdfs:range xsd:string .



###  http://www.sirma.com/ontologies/2016/02/culturalHeritageConservation/NGA#tradeName

nga:tradeName rdf:type owl:DatatypeProperty ;
              
              rdfs:label "Trade Name"@en ;
              
              dc:creator "Lidiya Dimitrova"@en ;
              
              skos:definition "Trade name of the product."@en ;
              
              rdfs:range xsd:string .



###  http://www.sirma.com/ontologies/2016/02/culturalHeritageConservation/NGA#treatmentType

nga:treatmentType rdf:type owl:DatatypeProperty ;
                  
                  rdfs:label "Treatment"@en ;
                  
                  skos:definition "Indicates if the treatment is minor or major."@en ;
                  
                  dc:creator "Lidiya Dimitrova"@en ;
                  
                  rdfs:range xsd:string .



###  http://www.sirma.com/ontologies/2016/02/culturalHeritageConservation/NGA#variableComponents

nga:variableComponents rdf:type owl:DatatypeProperty ;
                       
                       rdfs:label "Variable Components"@en ;
                       
                       skos:definition "Components that may be changed, such as a projector type, or may not be included in a given installation."@en ;
                       
                       dc:creator "Lidiya Dimitrova"@en ;
                       
                       rdfs:domain nga:Photograph ;
                       
                       rdfs:range xsd:string .



###  http://www.sirma.com/ontologies/2016/02/culturalHeritageConservation/NGA#vendorID

nga:vendorID rdf:type owl:DatatypeProperty ;
             
             rdfs:label "Vendor-ID"@en ;
             
             dc:creator "Lidiya Dimitrova"@en ;
             
             skos:definition "The identifier of the Vendor who sold the Frame."@en ;
             
             rdfs:domain nga:Frame ;
             
             rdfs:range xsd:string .



###  http://www.sirma.com/ontologies/2016/02/culturalHeritageConservation/NGA#vendorName

nga:vendorName rdf:type owl:DatatypeProperty ;
               
               rdfs:label "Vendor/Vendor Manufacturer"@en ;
               
               dc:creator "Lidiya Dimitrova"@en ;
               
               skos:definition "The name of the Vendor who sold the Frame."@en ;
               
               rdfs:range xsd:string .



###  http://www.sirma.com/ontologies/2016/02/culturalHeritageConservation/NGA#viewType

nga:viewType rdf:type owl:DatatypeProperty ;
             
             rdfs:label "View Type"@en ;
             
             skos:definition "Describes the vantage point of the image.."@en ;
             
             dc:creator "Lidiya Dimitrova"@en ;
             
             rdfs:domain emf:Image ;
             
             rdfs:range xsd:string .



###  http://www.sirma.com/ontologies/2016/02/culturalHeritageConservation/NGA#volume

nga:volume rdf:type owl:DatatypeProperty ;
           
           rdfs:label "Volume"@en ;
           
           dc:creator "Lidiya Dimitrova" ;
           
           skos:definition "The number of the volume in a set."@en ;
           
           rdfs:domain chc:CulturalObject ;
           
           rdfs:range xsd:string .



###  http://www.sirma.com/ontologies/2016/02/culturalHeritageConservation/NGA#volumeLanguage

nga:volumeLanguage rdf:type owl:DatatypeProperty ;
                   
                   rdfs:label "Language"@en ;
                   
                   dc:creator "Lidiya Dimitrova" ;
                   
                   skos:definition "The number of the volume, especially in a set."@en ;
                   
                   rdfs:domain chc:CulturalObject ;
                   
                   rdfs:range xsd:string .



###  http://www.sirma.com/ontologies/2016/02/culturalHeritageConservation/NGA#watermarks

nga:watermarks rdf:type owl:DatatypeProperty ;
               
               rdfs:label "Watermarks" ;
               
               skos:definition "Description of any watermarks evident in the paper/support."@en ;
               
               dc:creator "Lidiya Dimitrova"@en ;
               
               rdfs:domain chc:CulturalObject ;
               
               rdfs:range xsd:string .



###  http://www.sirma.com/ontologies/2016/02/culturalHeritageConservation/NGA#weaveDescription

nga:weaveDescription rdf:type owl:DatatypeProperty ;
                     
                     rdfs:label "Weave Description"@en ;
                     
                     skos:definition "A text description of different weave characteristics in the cultural object, making surface and substrate at the same time in textile or carpet. Might include fiber type, plys, spin, dyes used, etc."@en ;
                     
                     dc:creator "Lidiya Dimitrova"@en ;
                     
                     rdfs:domain chc:CulturalObject ;
                     
                     rdfs:range xsd:string .



###  http://www.sirma.com/ontologies/2016/02/culturalHeritageConservation/NGA#weight

nga:weight rdf:type owl:DatatypeProperty ;
           
           rdfs:label "Weight"@en ;
           
           skos:definition "Cultural object weight"@en ;
           
           dc:creator "Lidiya Dimitrova"@en ;
           
           rdfs:domain chc:CulturalObject ;
           
           rdfs:range xsd:string .





#################################################################
#
#    Classes
#
#################################################################


###  http://www.sirma.com/ontologies/2016/02/culturalHeritageConservation#CulturalObject

chc:CulturalObject emf:isSearchable "true"^^xsd:boolean .



###  http://www.sirma.com/ontologies/2016/02/culturalHeritageConservation#Sample

chc:Sample sec:allowInheritParentPermissions "false"^^xsd:boolean ;
           
           emf:isCreateable "true"^^xsd:boolean ;
           
           emf:isPartOfObjectLibrary "true"^^xsd:boolean ;
           
           sec:allowInheritLibraryPermissions "true"^^xsd:boolean ;
           
           emf:isSearchable "true"^^xsd:boolean .



###  http://www.sirma.com/ontologies/2016/02/culturalHeritageConservation/NGA#BoundVolume

nga:BoundVolume rdf:type owl:Class ;
                
                rdfs:label "Bound Volume"@en ;
                
                rdfs:subClassOf chc:CulturalObject ;
                
                sec:allowInheritParentPermissions "false"^^xsd:boolean ;
                
                sec:allowInheritLibraryPermissions "true"^^xsd:boolean ;
                
                emf:isPartOfObjectLibrary "true"^^xsd:boolean ;
                
                emf:isSearchable "true"^^xsd:boolean ;
                
                emf:isCreateable "true"^^xsd:boolean ;
                
                skos:definition "A volume is a bound collection of printed pages such as a book."@en ;
                
                dc:creator "Lidiya Dimitrova"@en .



###  http://www.sirma.com/ontologies/2016/02/culturalHeritageConservation/NGA#DecorativeArt

nga:DecorativeArt rdf:type owl:Class ;
                  
                  rdfs:label "Decorative Art"@en ;
                  
                  rdfs:subClassOf chc:CulturalObject ;
                  
                  sec:allowInheritParentPermissions "false"^^xsd:boolean ;
                  
                  sec:allowInheritLibraryPermissions "true"^^xsd:boolean ;
                  
                  emf:isSearchable "true"^^xsd:boolean ;
                  
                  emf:isCreateable "true"^^xsd:boolean ;
                  
                  emf:isPartOfObjectLibrary "true"^^xsd:boolean ;
                  
                  dc:creator "Lidiya Dimitrova"@en ;
                  
                  skos:definition "The decorative arts are arts or crafts concerned with the design and manufacture of beautiful objects that are also functional. It includes interior design, but not usually architecture . Examples include things like candle sticks, furniture, porcelain dinnerware, etc."@en .



###  http://www.sirma.com/ontologies/2016/02/culturalHeritageConservation/NGA#Drawing

nga:Drawing rdf:type owl:Class ;
            
            rdfs:label "Drawing"@en ;
            
            rdfs:subClassOf chc:CulturalObject ;
            
            sec:allowInheritParentPermissions "false"^^xsd:boolean ;
            
            emf:isPartOfObjectLibrary "true"^^xsd:boolean ;
            
            sec:allowInheritLibraryPermissions "true"^^xsd:boolean ;
            
            emf:isSearchable "true"^^xsd:boolean ;
            
            emf:isCreateable "true"^^xsd:boolean ;
            
            skos:definition "Drawing is a form of visual art that makes use of any number of drawing instruments to mark a two-dimensional medium. Instruments used include graphite pencils, pen and ink, inked brushes, wax color pencils, crayons, charcoal, chalk, pastels, various kinds of erasers, markers, styluses, and various metals (such as silverpoint) (Wikipedia)"@en ;
            
            dc:creator "Kiril Penev"@en .



###  http://www.sirma.com/ontologies/2016/02/culturalHeritageConservation/NGA#Ephemera

nga:Ephemera rdf:type owl:Class ;
             
             rdfs:label "Ephemera" ;
             
             rdfs:subClassOf chc:CulturalObject ;
             
             sec:allowInheritParentPermissions "false"^^xsd:boolean ;
             
             emf:isSearchable "true"^^xsd:boolean ;
             
             emf:isCreateable "true"^^xsd:boolean ;
             
             emf:isPartOfObjectLibrary "true"^^xsd:boolean ;
             
             sec:allowInheritLibraryPermissions "true"^^xsd:boolean ;
             
             dc:creator "Lidiya Dimitrova" ;
             
             skos:definition "Ephemera are any transitory written or printed matter meant for eventual repression (or not meant to be retained or preserved). However in the museum or archives context, ephemera must be preserved and accounted for." .



###  http://www.sirma.com/ontologies/2016/02/culturalHeritageConservation/NGA#Frame

nga:Frame rdf:type owl:Class ;
          
          rdfs:label "Frame"@en ;
          
          rdfs:subClassOf chc:CulturalObject ;
          
          sec:allowInheritParentPermissions "false"^^xsd:boolean ;
          
          emf:isSearchable "true"^^xsd:boolean ;
          
          sec:allowInheritLibraryPermissions "true"^^xsd:boolean ;
          
          emf:isPartOfObjectLibrary "true"^^xsd:boolean ;
          
          emf:isCreateable "true"^^xsd:boolean ;
          
          skos:definition "A frame is a decorative molding that typically is attached to a painting or other cultural object especially when that cultural object is displayed. It typically surrounds and covers the edges of the cultural object. It is typically made of wood/plaster/gold leaf, but can be any material."@en ;
          
          dc:creator "Lidiya Dimitrova"@en .



###  http://www.sirma.com/ontologies/2016/02/culturalHeritageConservation/NGA#MediaArt

nga:MediaArt rdf:type owl:Class ;
             
             rdfs:label "Media Art"@en ;
             
             rdfs:subClassOf chc:CulturalObject ;
             
             sec:allowInheritParentPermissions "false"^^xsd:boolean ;
             
             emf:isSearchable "true"^^xsd:boolean ;
             
             sec:allowInheritLibraryPermissions "true"^^xsd:boolean ;
             
             emf:isPartOfObjectLibrary "true"^^xsd:boolean ;
             
             emf:isCreateable "true"^^xsd:boolean ;
             
             dc:creator "Lidiya Dimitrova"@en ;
             
             skos:definition "Media art is a genre that encompasses artworks created with new media technologies, including digital art, computer animation, computer graphics, virtual art, internet art, interactive art, video games, computer robotics, 3-D printing, and art as biotechnology. It can also include film if not represented elsewhere."@en .



###  http://www.sirma.com/ontologies/2016/02/culturalHeritageConservation/NGA#Painting

nga:Painting rdf:type owl:Class ;
             
             rdfs:label "Painting"@en ;
             
             rdfs:subClassOf chc:CulturalObject ;
             
             sec:allowInheritParentPermissions "false"^^xsd:boolean ;
             
             emf:isCreateable "true"^^xsd:boolean ;
             
             emf:isSearchable "true"^^xsd:boolean ;
             
             emf:isPartOfObjectLibrary "true"^^xsd:boolean ;
             
             sec:allowInheritLibraryPermissions "true"^^xsd:boolean ;
             
             dc:creator "Kiril Penev"@en ;
             
             skos:definition "Painting is the practice of applying paint, pigment, color or other medium to a surface (support base). The medium is commonly applied to the base with a brush but other implements, such as knives, sponges, and airbrushes, can be used. In art, the term painting describes both the act and the result of the action. However, painting is also used outside of art as a common trade among craftsmen and builders. Paintings may have for their support such surfaces as walls, paper, canvas, wood, glass, lacquer, clay, leaf, copper or concrete, and may incorporate multiple other materials including sand, clay, paper, gold leaf as well as objects. (Wikipedia)"@en .



###  http://www.sirma.com/ontologies/2016/02/culturalHeritageConservation/NGA#Photograph

nga:Photograph rdf:type owl:Class ;
               
               rdfs:label "Photograph"@en ;
               
               rdfs:subClassOf chc:CulturalObject ;
               
               sec:allowInheritParentPermissions "false"^^xsd:boolean ;
               
               emf:isSearchable "true"^^xsd:boolean ;
               
               emf:isCreateable "true"^^xsd:boolean ;
               
               sec:allowInheritLibraryPermissions "true"^^xsd:boolean ;
               
               emf:isPartOfObjectLibrary "true"^^xsd:boolean ;
               
               skos:definition "A photograph or photo is an image created by light falling on a light-sensitive surface, usually photographic film or an electronic image such as a CCD or a CMOS chip. Most photographs are created using a camera, which uses a lens to focus the scene's visible wavelengths of light into a reproduction of what the human eye would see. (Wikipedia)"@en ;
               
               dc:creator "Kiril Penev"@en .



###  http://www.sirma.com/ontologies/2016/02/culturalHeritageConservation/NGA#Portfolio

nga:Portfolio rdf:type owl:Class ;
              
              rdfs:label "Portfolio"@en ;
              
              rdfs:subClassOf chc:CulturalObject ;
              
              sec:allowInheritParentPermissions "false"^^xsd:boolean ;
              
              sec:allowInheritLibraryPermissions "true"^^xsd:boolean ;
              
              emf:isCreateable "true"^^xsd:boolean ;
              
              emf:isSearchable "true"^^xsd:boolean ;
              
              emf:isPartOfObjectLibrary "true"^^xsd:boolean ;
              
              skos:definition "A portfolio is an edited collection of artwork. It usually has a cover or housing to keep the collection together. "@en ;
              
              dc:creator "Lidiya Dimitrova"@en .



###  http://www.sirma.com/ontologies/2016/02/culturalHeritageConservation/NGA#Print

nga:Print rdf:type owl:Class ;
          
          rdfs:label "Print"@en ;
          
          rdfs:subClassOf chc:CulturalObject ;
          
          sec:allowInheritParentPermissions "false"^^xsd:boolean ;
          
          emf:isCreateable "true"^^xsd:boolean ;
          
          sec:allowInheritLibraryPermissions "true"^^xsd:boolean ;
          
          emf:isPartOfObjectLibrary "true"^^xsd:boolean ;
          
          emf:isSearchable "true"^^xsd:boolean ;
          
          skos:definition """A picture or design printed from a block or plate or copied from a painting by photography.
A piece of fabric or clothing with a decorative colored pattern or design printed on it."""@en ;
          
          dc:creator "Kiril Penev"@en .



###  http://www.sirma.com/ontologies/2016/02/culturalHeritageConservation/NGA#Sculpture

nga:Sculpture rdf:type owl:Class ;
              
              rdfs:label "Sculpture"@en ;
              
              rdfs:subClassOf chc:CulturalObject ;
              
              sec:allowInheritParentPermissions "false"^^xsd:boolean ;
              
              emf:isPartOfObjectLibrary "true"^^xsd:boolean ;
              
              emf:isCreateable "true"^^xsd:boolean ;
              
              emf:isSearchable "true"^^xsd:boolean ;
              
              sec:allowInheritLibraryPermissions "true"^^xsd:boolean ;
              
              dc:creator "Kiril Penev"@en ;
              
              skos:definition "Sculpture is the branch of the visual arts that operates in three dimensions, and one of the plastic arts. Durable sculptural processes originally used carving (the removal of material) and modelling (the addition of material, as clay), in stone, metal, ceramics, wood and other materials but, since modernism, shifts in sculptural process led to an almost complete freedom of materials and process. A wide variety of materials may be worked by removal such as carving, assembled by welding or modelling, or molded, or cast. (Wikipedia)"@en .



###  http://www.sirma.com/ontologies/2016/02/culturalHeritageConservation/NGA#TechnicalMaterial

nga:TechnicalMaterial rdf:type owl:Class ;
                      
                      rdfs:label "Technical Material"@en ;
                      
                      rdfs:subClassOf chc:CulturalObject ;
                      
                      sec:allowInheritParentPermissions "false"^^xsd:boolean ;
                      
                      sec:allowInheritLibraryPermissions "true"^^xsd:boolean ;
                      
                      emf:isCreateable "true"^^xsd:boolean ;
                      
                      emf:isSearchable "true"^^xsd:boolean ;
                      
                      emf:isPartOfObjectLibrary "true"^^xsd:boolean ;
                      
                      dc:creator "Lidiya Dimitrova"@en ;
                      
                      skos:definition "Technical Material (in the context of the NGA's collection management system (TMS)) are accessioned cultural objects that are related to the production of works of art. The best example of these types of materials are metal plates, usually copper, that have been etched or engraved by the artist in order to make a series of prints on paper. Another example could be a mold that an artist made to cast a series of three dimensional sculptures."@en .





#################################################################
#
#    Annotations
#
#################################################################


chc:documents emf:isSearchable "true"^^xsd:boolean .



chc:isDocumentedIn emf:isSearchable "true"^^xsd:boolean .



emf:hasWatcher emf:auditEvent "+addHasWatcher|-removeHasWatcher|changeHasWatcher" ;
               
               sec:autoAssignPermissionRole "CONSUMER" .



chc:hasDepiction emf:isSearchable "true"^^xsd:boolean .



emf:isPrimaryImageOf emf:isSearchable "true"^^xsd:boolean ;
                     
                     emf:auditEvent "+addIsPrimaryImageOf|-removeIsPrimaryImageOf|changeIsPrimaryImageOf" .



chc:hasAuthor emf:isSearchable "true"^^xsd:boolean ;
              
              sec:autoAssignPermissionRole "COLLABORATOR" ;
              
              sec:autoAssignParentPermissionRole "CONSUMER" .



chc:attachmentOf emf:isSearchable "true"^^xsd:boolean .



chc:hasAttachment emf:isSearchable "true"^^xsd:boolean .



chc:depicts emf:isSearchable "true"^^xsd:boolean .



chc:approvedBy emf:isSearchable "true"^^xsd:boolean ;
               
               sec:autoAssignPermissionRole "COLLABORATOR" ;
               
               sec:autoAssignParentPermissionRole "CONSUMER" .



ptop:involvedIn emf:isSearchable "true"^^xsd:boolean ;
                
                emf:auditEvent "+addInvolvedIn|-removeInvolvedIn|changeInvolvedIn" .



chc:hasApproved emf:isSearchable "true"^^xsd:boolean .



chc:duplicates emf:isSearchable "true"^^xsd:boolean .



emf:hasAssignee sec:autoAssignParentPermissionRole "COLLABORATOR" ;
                
                sec:autoAssignPermissionRole "COLLABORATOR" .



emf:isWatcherOf emf:auditEvent "+addIsWatcherOf|-removeIsWatcherOf|changeIsWatcherOf" .



emf:processedBy emf:isSearchable "true"^^xsd:boolean ;
                
                emf:auditEvent "+addProcessedBy|-removeProcessedBy|changeProcessedBy" .



chc:isAuthorOf emf:isSearchable "true"^^xsd:boolean .



chc:hasSupervisor emf:isSearchable "true"^^xsd:boolean ;
                  
                  sec:autoAssignParentPermissionRole "COLLABORATOR" ;
                  
                  sec:autoAssignPermissionRole "COLLABORATOR" .



chc:hasSample emf:isSearchable "true"^^xsd:boolean .



chc:isTakenFrom emf:isSearchable "true"^^xsd:boolean .



chc:ConservationActivity sec:allowInheritLibraryPermissions "false"^^xsd:boolean ;
                         
                         emf:isCreateable "true"^^xsd:boolean ;
                         
                         sec:allowInheritParentPermissions "true"^^xsd:boolean ;
                         
                         emf:isPartOfObjectLibrary "true"^^xsd:boolean ;
                         
                         emf:isSearchable "true"^^xsd:boolean .



emf:hasPrimaryImage emf:isSearchable "true"^^xsd:boolean ;
                    
                    emf:auditEvent "+addHasPrimaryImage|-removeHasPrimaryImage|changeHasPrimaryImage" .



chc:isSupervisorOf emf:isSearchable "true"^^xsd:boolean .



emf:processes emf:isSearchable "true"^^xsd:boolean ;
              
              emf:auditEvent "+addProcesses|-removeProcesses|changeProcesses" .



ptop:hasParticipant emf:isSearchable "true"^^xsd:boolean ;
                    
                    sec:autoAssignPermissionRole "COLLABORATOR" ;
                    
                    sec:autoAssignParentPermissionRole "COLLABORATOR" ;
                    
                    emf:auditEvent "+addHasParticipant|-removeHasParticipant|changeHasParticipant" .




###  Generated by the OWL API (version 3.4.2) http://owlapi.sourceforge.net

