@prefix : <http://www.semanticweb.org/owl/owlapi/turtle#> .
@prefix dc: <http://purl.org/dc/elements/1.1/> .
@prefix chc: <http://www.sirma.com/ontologies/2016/02/culturalHeritageConservation#> .
@prefix emf: <http://ittruse.ittbg.com/ontology/enterpriseManagementFramework#> .
@prefix ima: <http://www.sirma.com/ontologies/2016/02/culturalHeritageConservation/IMA#> .
@prefix owl: <http://www.w3.org/2002/07/owl#> .
@prefix rdf: <http://www.w3.org/1999/02/22-rdf-syntax-ns#> .
@prefix xml: <http://www.w3.org/XML/1998/namespace> .
@prefix xsd: <http://www.w3.org/2001/XMLSchema#> .
@prefix ptop: <http://www.ontotext.com/proton/protontop#> .
@prefix rdfs: <http://www.w3.org/2000/01/rdf-schema#> .
@prefix skos: <http://www.w3.org/2004/02/skos/core#> .
@prefix dcterms: <http://purl.org/dc/terms/> .
@base <http://www.sirma.com/ontologies/2016/02/culturalHeritageConservation/IMA> .

<http://www.sirma.com/ontologies/2016/02/culturalHeritageConservation/IMA> rdf:type owl:Ontology ;
                                                                           
                                                                           rdfs:label "Extension of Cultural Heritage Conservation Ontology Model for IMA"@en ;
                                                                           
                                                                           owl:versionInfo "0.1"@en ;
                                                                           
                                                                           dc:subject "Extension of Cultural Heritage Conservation Ontology Model for IMA"@en ;
                                                                           
                                                                           rdfs:comment "IMA Extension of Cultural Heritage Conservation Ontology Model for Conservation Space project"@en ;
                                                                           
                                                                           dc:creator "Lidiya Dimitrova"@en ;
                                                                           
                                                                           owl:imports <http://www.sirma.com/ontologies/2016/02/culturalHeritageConservation> .


#################################################################
#
#    Object Properties
#
#################################################################


###  http://www.sirma.com/ontologies/2016/02/culturalHeritageConservation/IMA#duplicates

ima:duplicates rdf:type owl:ObjectProperty ,
                        owl:SymmetricProperty ;
               
               rdfs:label "Duplicates"@en ;
               
               emf:isSearchable "true"^^xsd:boolean ;
               
               dc:creator "Lidiya Dimitrova" ;
               
               skos:definition "Indicates that the cultural object duplicates another cultural object."@en ;
               
               rdfs:domain chc:CulturalObject ;
               
               rdfs:range chc:CulturalObject .





#################################################################
#
#    Data properties
#
#################################################################


###  http://www.sirma.com/ontologies/2016/02/culturalHeritageConservation/IMA#accessionNumber

ima:accessionNumber rdf:type owl:DatatypeProperty ;
                    
                    rdfs:label "Accession Number"@en ;
                    
                    dc:creator "Lidiya Dimitrova"@en ;
                    
                    skos:definition "Unique institutional ID. Can be coded to be human readable and to express, for example, year/lot/number if acquisition or shelf location"@en ;
                    
                    rdfs:domain chc:CulturalObject ;
                    
                    rdfs:range xsd:string .



###  http://www.sirma.com/ontologies/2016/02/culturalHeritageConservation/IMA#aestheticPriority

ima:aestheticPriority rdf:type owl:DatatypeProperty ;
                      
                      rdfs:label "Aesthetic Priority"@en ;
                      
                      skos:definition "Aesthetic appearance determines priority for treatment"@en ;
                      
                      dc:creator "Lidiya Dimitrova"@en ;
                      
                      rdfs:domain chc:CulturalObject ;
                      
                      rdfs:range xsd:string .



###  http://www.sirma.com/ontologies/2016/02/culturalHeritageConservation/IMA#artistInstructions

ima:artistInstructions rdf:type owl:DatatypeProperty ;
                       
                       rdfs:label "Artist Instructions"@en ;
                       
                       skos:definition "Artists description of how the work is to be displayed/installed"@en ;
                       
                       dc:creator "Lidiya Dimitrova"@en ;
                       
                       rdfs:domain chc:CulturalObject ;
                       
                       rdfs:range xsd:string .



###  http://www.sirma.com/ontologies/2016/02/culturalHeritageConservation/IMA#artistNames

ima:artistNames rdf:type owl:DatatypeProperty ;
                
                rdfs:label "Artist/Maker"@en ;
                
                skos:definition "An entity primarily responsible for creating an object"@en ;
                
                dc:creator "Lidiya Dimitrova"@en ;
                
                rdfs:domain chc:CulturalObject ;
                
                rdfs:range xsd:string .



###  http://www.sirma.com/ontologies/2016/02/culturalHeritageConservation/IMA#associatedMaterials

ima:associatedMaterials rdf:type owl:DatatypeProperty ;
                        
                        rdfs:label "Associated Materials"@en ;
                        
                        dc:creator "Lidiya Dimitrova"@en ;
                        
                        skos:definition "This would include materials provided by the artist that are used for installation/adjustment/repair of the work of art, but are not actually part of the work of art."@en ;
                        
                        rdfs:domain chc:CulturalObject ;
                        
                        rdfs:range xsd:string .



###  http://www.sirma.com/ontologies/2016/02/culturalHeritageConservation/IMA#attachmentDescription

ima:attachmentDescription rdf:type owl:DatatypeProperty ;
                          
                          rdfs:label "Attachment Description"@en ;
                          
                          dc:creator "Lidiya Dimitrova"@en ;
                          
                          skos:definition "Text description of how  the object is attached to the mat. (attachment method). Example: hinges, inlay"@en ;
                          
                          rdfs:domain chc:CulturalObject ;
                          
                          rdfs:range xsd:string .



###  http://www.sirma.com/ontologies/2016/02/culturalHeritageConservation/IMA#auxiliaryComponents

ima:auxiliaryComponents rdf:type owl:DatatypeProperty ;
                        
                        rdfs:label "Auxiliary Components"@en ;
                        
                        dc:creator "Lidiya Dimitrova"@en ;
                        
                        skos:definition "Non-attached associated components"@en ;
                        
                        rdfs:domain chc:CulturalObject ;
                        
                        rdfs:range xsd:string .



###  http://www.sirma.com/ontologies/2016/02/culturalHeritageConservation/IMA#baseDescription

ima:baseDescription rdf:type owl:DatatypeProperty ;
                    
                    rdfs:label "Base Description"@en ;
                    
                    dc:creator "Lidiya Dimitrova"@en ;
                    
                    skos:definition "The bottom support of anything; that on which a thing stands or rests"@en ;
                    
                    rdfs:domain chc:CulturalObject ;
                    
                    rdfs:range xsd:string .



###  http://www.sirma.com/ontologies/2016/02/culturalHeritageConservation/IMA#century

ima:century rdf:type owl:DatatypeProperty ;
            
            rdfs:label "Century"@en ;
            
            dc:creator "Lidiya Dimitrova"@en ;
            
            skos:definition "The century when the cultural object is created."@en ;
            
            rdfs:domain ima:Frame ;
            
            rdfs:range xsd:string .



###  http://www.sirma.com/ontologies/2016/02/culturalHeritageConservation/IMA#conservationStatus

ima:conservationStatus rdf:type owl:DatatypeProperty ;
                       
                       rdfs:label "Conservation Status"@en ;
                       
                       skos:definition "General statement of condition."@en ;
                       
                       dc:creator "Lidiya Dimitrova"@en ;
                       
                       rdfs:domain chc:CulturalObject ;
                       
                       rdfs:subPropertyOf chc:condition ;
                       
                       rdfs:range xsd:string .



###  http://www.sirma.com/ontologies/2016/02/culturalHeritageConservation/IMA#construction

ima:construction rdf:type owl:DatatypeProperty ;
                 
                 rdfs:label "Construction"@en ;
                 
                 dc:creator "Lidiya Dimitrova"@en ;
                 
                 skos:definition "Weave Structure,machine or hand sewn, previously repaired or altered, opening placement and construction (i.e. zipper on proper left)"@en ;
                 
                 rdfs:domain chc:CulturalObject ;
                 
                 rdfs:range xsd:string .



###  http://www.sirma.com/ontologies/2016/02/culturalHeritageConservation/IMA#creationDates

ima:creationDates rdf:type owl:DatatypeProperty ;
                  
                  rdfs:label "Creation Date"@en ;
                  
                  dc:creator "Lidiya Dimitrova"@en ;
                  
                  skos:definition "Start/end dates and qualifiers such as \"circa\", \"before\", etc. Can have historical records of former attributions of creation dates."@en ;
                  
                  rdfs:domain chc:CulturalObject ;
                  
                  rdfs:range xsd:string .



###  http://www.sirma.com/ontologies/2016/02/culturalHeritageConservation/IMA#curatorialDepartment

ima:curatorialDepartment rdf:type owl:DatatypeProperty ;
                         
                         rdfs:label "Curatorial Department"@en ;
                         
                         skos:definition """Departments responsible for the Object. 
They are responsible for the curatorial management and displaying for exhibition but acquisition is done by Registrar office."""@en ;
                         
                         dc:creator "Lidiya Dimitrova"@en ;
                         
                         rdfs:domain chc:CulturalObject ;
                         
                         rdfs:range xsd:string .



###  http://www.sirma.com/ontologies/2016/02/culturalHeritageConservation/IMA#designHouse

ima:designHouse rdf:type owl:DatatypeProperty ;
                
                rdfs:label "Design House"@en ;
                
                dc:creator "Lidiya Dimitrova"@en ;
                
                skos:definition "Outer dimensions of the framed or unframed work when installed."@en ;
                
                rdfs:domain chc:CulturalObject ;
                
                rdfs:range xsd:string .



###  http://www.sirma.com/ontologies/2016/02/culturalHeritageConservation/IMA#designerNames

ima:designerNames rdf:type owl:DatatypeProperty ;
                  
                  rdfs:label "Designer"@en ;
                  
                  dc:creator "Lidiya Dimitrova"@en ;
                  
                  skos:definition "Name of the costume designer."@en ;
                  
                  rdfs:domain chc:CulturalObject ;
                  
                  rdfs:range xsd:string .



###  http://www.sirma.com/ontologies/2016/02/culturalHeritageConservation/IMA#displayDimensions

ima:displayDimensions rdf:type owl:DatatypeProperty ;
                      
                      rdfs:label "Display Dimensions"@en ;
                      
                      dc:creator "Lidiya Dimitrova"@en ;
                      
                      skos:definition "Outer dimensions of the framed or unframed work when installed."@en ;
                      
                      rdfs:domain chc:CulturalObject ;
                      
                      rdfs:range xsd:string .



###  http://www.sirma.com/ontologies/2016/02/culturalHeritageConservation/IMA#displayRequirement

ima:displayRequirement rdf:type owl:DatatypeProperty ;
                       
                       rdfs:label "Display Requirement"@en ;
                       
                       skos:definition "Environmental requirements as well as how to display the cultural object."@en ;
                       
                       dc:creator "Lidiya Dimitrova"@en ;
                       
                       rdfs:range xsd:string .



###  http://www.sirma.com/ontologies/2016/02/culturalHeritageConservation/IMA#essentialComponents

ima:essentialComponents rdf:type owl:DatatypeProperty ;
                        
                        rdfs:label "Essential Components"@en ;
                        
                        dc:creator "Lidiya Dimitrova"@en ;
                        
                        skos:definition "These are the parts of the artwork that artist indicates cannot be changed or replaced."@en ;
                        
                        rdfs:domain chc:CulturalObject ;
                        
                        rdfs:range xsd:string .



###  http://www.sirma.com/ontologies/2016/02/culturalHeritageConservation/IMA#estimatedHours

ima:estimatedHours rdf:type owl:DatatypeProperty ;
                   
                   rdfs:label "Estimated Hours"@en ;
                   
                   dc:creator "Lidiya Dimitrova"@en ;
                   
                   skos:definition "Number of hours estimated to complete the treatment - linked to CMS Condition tab."@en ;
                   
                   rdfs:range xsd:string .



###  http://www.sirma.com/ontologies/2016/02/culturalHeritageConservation/IMA#fabricationDescription

ima:fabricationDescription rdf:type owl:DatatypeProperty ;
                           
                           rdfs:label "Fabrication Description"@en ;
                           
                           skos:definition "Description of the fabrication method of the art object."@en ;
                           
                           dc:creator "Lidiya Dimitrova"@en ;
                           
                           rdfs:domain chc:CulturalObject ;
                           
                           rdfs:range xsd:string .



###  http://www.sirma.com/ontologies/2016/02/culturalHeritageConservation/IMA#fabricationMethod

ima:fabricationMethod rdf:type owl:DatatypeProperty ;
                      
                      rdfs:label "Fabrication Description"@en ;
                      
                      skos:definition "Description of the fabrication method of the art object."@en ;
                      
                      dc:creator "Lidiya Dimitrova"@en ;
                      
                      rdfs:domain chc:CulturalObject ;
                      
                      rdfs:range xsd:string .



###  http://www.sirma.com/ontologies/2016/02/culturalHeritageConservation/IMA#frameCountry

ima:frameCountry rdf:type owl:DatatypeProperty ;
                 
                 rdfs:label "Country/Region"@en ;
                 
                 skos:definition "Certain frame styles are synonymous with a certain country."@en ;
                 
                 dc:creator "Lidiya Dimitrova"@en ;
                 
                 rdfs:domain ima:Frame ;
                 
                 rdfs:range xsd:string .



###  http://www.sirma.com/ontologies/2016/02/culturalHeritageConservation/IMA#frameDescription

ima:frameDescription rdf:type owl:DatatypeProperty ;
                     
                     rdfs:label "Frame Description"@en ;
                     
                     dc:creator "Lidiya Dimitrova"@en ;
                     
                     skos:definition "Text description of the frame if part of the original art object. example Tuttle. or if the object is permanently framed in storage. Include glazing, framing package and backing."@en ;
                     
                     rdfs:domain chc:CulturalObject ;
                     
                     rdfs:range xsd:string .



###  http://www.sirma.com/ontologies/2016/02/culturalHeritageConservation/IMA#generalAccessories

ima:generalAccessories rdf:type owl:DatatypeProperty ;
                       
                       rdfs:label "Accessories"@en ;
                       
                       dc:creator "Lidiya Dimitrova"@en ;
                       
                       skos:definition "Objects associated with a cultural object. Such as a special hanging bracket, a diagram for safely installing, or a videotape for safely installing, also a special grease for a machine that is part of the cultural object."@en ;
                       
                       rdfs:domain chc:CulturalObject ;
                       
                       rdfs:range xsd:string .



###  http://www.sirma.com/ontologies/2016/02/culturalHeritageConservation/IMA#generalCondition

ima:generalCondition rdf:type owl:DatatypeProperty ;
                     
                     rdfs:label "Condition"@en ;
                     
                     skos:definition " Very general text description of condition"@en ;
                     
                     dc:creator "Lidiya Dimitrova"@en ;
                     
                     rdfs:subPropertyOf chc:condition ;
                     
                     rdfs:range xsd:string .



###  http://www.sirma.com/ontologies/2016/02/culturalHeritageConservation/IMA#glazingDescription

ima:glazingDescription rdf:type owl:DatatypeProperty ;
                       
                       rdfs:label "Glazing Description"@en ;
                       
                       dc:creator "Lidiya Dimitrova"@en ;
                       
                       skos:definition "The text description of unusual glazing requirement such as Optium for a friable drawing."@en ;
                       
                       rdfs:domain chc:CulturalObject ;
                       
                       rdfs:range xsd:string .



###  http://www.sirma.com/ontologies/2016/02/culturalHeritageConservation/IMA#handlingRequirements

ima:handlingRequirements rdf:type owl:DatatypeProperty ;
                         
                         rdfs:label "Handling Requirement"@en ;
                         
                         skos:definition "Handling specifications"@en ;
                         
                         dc:creator "Lidiya Dimitrova"@en ;
                         
                         rdfs:range xsd:string .



###  http://www.sirma.com/ontologies/2016/02/culturalHeritageConservation/IMA#homeLocation

ima:homeLocation rdf:type owl:DatatypeProperty ;
                 
                 rdfs:label "Home Location"@en ;
                 
                 dc:creator "Lidiya Dimitrova"@en ;
                 
                 skos:definition "Location could be a gallery or storage location where the cultural object normally is"@en ;
                 
                 rdfs:domain chc:CulturalObject ;
                 
                 rdfs:range xsd:string .



###  http://www.sirma.com/ontologies/2016/02/culturalHeritageConservation/IMA#housingDescription

ima:housingDescription rdf:type owl:DatatypeProperty ;
                       
                       rdfs:label "Housing Description"@en ;
                       
                       dc:creator "Lidiya Dimitrova"@en ;
                       
                       skos:definition "Text describing   permanent housing when it is in storage. example: A box for the rolled Escher Genesis"@en ;
                       
                       rdfs:domain chc:CulturalObject ;
                       
                       rdfs:range xsd:string .



###  http://www.sirma.com/ontologies/2016/02/culturalHeritageConservation/IMA#imageDetail

ima:imageDetail rdf:type owl:DatatypeProperty ;
                
                rdfs:label "Detail"@en ;
                
                skos:definition "Image details"@en ;
                
                dc:creator "Lidiya Dimitrova"@en ;
                
                rdfs:domain emf:Image ;
                
                rdfs:range xsd:string .



###  http://www.sirma.com/ontologies/2016/02/culturalHeritageConservation/IMA#imageLightingCondition

ima:imageLightingCondition rdf:type owl:DatatypeProperty ;
                           
                           rdfs:label "Lighting Condition"@en ;
                           
                           dc:creator "Lidiya Dimitrova"@en ;
                           
                           skos:definition "Lighting Condition of the image"@en ;
                           
                           rdfs:domain emf:Image ;
                           
                           rdfs:range xsd:string .



###  http://www.sirma.com/ontologies/2016/02/culturalHeritageConservation/IMA#imageShotDate

ima:imageShotDate rdf:type owl:DatatypeProperty ;
                  
                  rdfs:label "Date Shot"@en ;
                  
                  dc:creator "Lidiya Dimitrova"@en ;
                  
                  skos:definition "The date the image was made"@en ;
                  
                  rdfs:domain emf:Image ;
                  
                  rdfs:range xsd:dateTime .



###  http://www.sirma.com/ontologies/2016/02/culturalHeritageConservation/IMA#innerDimensions

ima:innerDimensions rdf:type owl:DatatypeProperty ;
                    
                    rdfs:label "Inner Dimensions"@en ;
                    
                    skos:definition "Inside dimension of the Frame (Text height and width)"@en ;
                    
                    dc:creator "Lidiya Dimitrova"@en ;
                    
                    rdfs:domain ima:Frame ;
                    
                    rdfs:range xsd:string .



###  http://www.sirma.com/ontologies/2016/02/culturalHeritageConservation/IMA#inscriptions

ima:inscriptions rdf:type owl:DatatypeProperty ;
                 
                 rdfs:label "Inscription(s)"@en ;
                 
                 skos:definition "Free text description of any writing or printing on the object's obverse or reverse. Artist signature, dealer marks, inventory codes, etc."@en ;
                 
                 dc:creator "Lidiya Dimitrova"@en ;
                 
                 rdfs:domain chc:CulturalObject ;
                 
                 rdfs:range xsd:dateTime .



###  http://www.sirma.com/ontologies/2016/02/culturalHeritageConservation/IMA#installationInstruction

ima:installationInstruction rdf:type owl:DatatypeProperty ;
                            
                            rdfs:label "Installation Instruction"@en ;
                            
                            dc:creator "Lidiya Dimitrova"@en ;
                            
                            skos:definition "Text of any special Installation Instruction that the cultural object may require"@en ;
                            
                            rdfs:domain ima:Frame ;
                            
                            rdfs:range xsd:string .



###  http://www.sirma.com/ontologies/2016/02/culturalHeritageConservation/IMA#labelRequirement

ima:labelRequirement rdf:type owl:DatatypeProperty ;
                     
                     rdfs:label "Label Requirement"@en ;
                     
                     dc:creator "Lidiya Dimitrova"@en ;
                     
                     skos:definition "Type and placement of an accession number label"@en ;
                     
                     rdfs:range xsd:string .



###  http://www.sirma.com/ontologies/2016/02/culturalHeritageConservation/IMA#loanRequirements

ima:loanRequirements rdf:type owl:DatatypeProperty ;
                     
                     rdfs:label "Loan Requirement"@en ;
                     
                     skos:definition "Costume: Can the costume be loaned or not, and if yes, what are the requirements for packing and shipping - linked to CMS Catalogue Module Recommend Tab
Costume Accessory: Can the costume accessory be loaned or not, and if yes, what are the requirements for packing and shipping -  linked to CMS Catalogue Module Recommend Tab"@en ;
                     
                     dc:creator "Lidiya Dimitrova"@en ;
                     
                     rdfs:range xsd:string .



###  http://www.sirma.com/ontologies/2016/02/culturalHeritageConservation/IMA#manufactureMethod

ima:manufactureMethod rdf:type owl:DatatypeProperty ;
                      
                      rdfs:label "Method Of Manufacture"@en ;
                      
                      dc:creator "Lidiya Dimitrova"@en ;
                      
                      skos:definition "More specific details of how an object is made based on examination."@en ;
                      
                      rdfs:domain chc:CulturalObject ;
                      
                      rdfs:range xsd:string .



###  http://www.sirma.com/ontologies/2016/02/culturalHeritageConservation/IMA#marks

ima:marks rdf:type owl:DatatypeProperty ;
          
          rdfs:label "Marks"@en ;
          
          skos:definition "Description of any marks not related to the image such notations or marks made by a processes"@en ;
          
          dc:creator "Lidiya Dimitrova"@en ;
          
          rdfs:domain chc:CulturalObject ;
          
          rdfs:range xsd:string .



###  http://www.sirma.com/ontologies/2016/02/culturalHeritageConservation/IMA#matType

ima:matType rdf:type owl:DatatypeProperty ;
            
            rdfs:label "Mat Type"@en ;
            
            dc:creator "Lidiya Dimitrova"@en ;
            
            skos:definition "Text description of the mat, specially unusual ones such as deep mat with wrapper for pastel."@en ;
            
            rdfs:domain chc:CulturalObject ;
            
            rdfs:range xsd:string .



###  http://www.sirma.com/ontologies/2016/02/culturalHeritageConservation/IMA#materials

ima:materials rdf:type owl:DatatypeProperty ;
              
              rdfs:label "Materials"@en ;
              
              skos:definition "All of the materials used to create the textile, costume, needlework."@en ;
              
              dc:creator "Lidiya Dimitrova" ;
              
              rdfs:domain chc:CulturalObject ;
              
              rdfs:range xsd:string .



###  http://www.sirma.com/ontologies/2016/02/culturalHeritageConservation/IMA#mediaDescription

ima:mediaDescription rdf:type owl:DatatypeProperty ;
                     
                     rdfs:label "Media Description"@en ;
                     
                     dc:creator "Lidiya Dimitrova" ;
                     
                     skos:definition "Text description of the media used for the drawing(graphite, chalk, pen & ink)."@en ;
                     
                     rdfs:domain chc:CulturalObject ;
                     
                     rdfs:range xsd:string .



###  http://www.sirma.com/ontologies/2016/02/culturalHeritageConservation/IMA#medium

ima:medium rdf:type owl:DatatypeProperty ;
           
           rdfs:label "Medium and Support"@en ;
           
           dc:creator "Lidiya Dimitrova" ;
           
           skos:definition "Medium description often used for public"@en ;
           
           rdfs:domain chc:CulturalObject ;
           
           rdfs:range xsd:string .



###  http://www.sirma.com/ontologies/2016/02/culturalHeritageConservation/IMA#moldingWidth

ima:moldingWidth rdf:type owl:DatatypeProperty ;
                 
                 rdfs:label "Molding Width"@en ;
                 
                 dc:creator "Lidiya Dimitrova" ;
                 
                 skos:definition "The measurement from the site edge to the outer edge of the frame"@en ;
                 
                 rdfs:domain ima:Frame ;
                 
                 rdfs:range xsd:string .



###  http://www.sirma.com/ontologies/2016/02/culturalHeritageConservation/IMA#mountDescription

ima:mountDescription rdf:type owl:DatatypeProperty ;
                     
                     rdfs:label "Mount Description"@en ;
                     
                     dc:creator "Lidiya Dimitrova"@en ;
                     
                     skos:definition "Text description of the mounting when Art objects is on display"@en ;
                     
                     rdfs:domain chc:CulturalObject ;
                     
                     rdfs:range xsd:string .



###  http://www.sirma.com/ontologies/2016/02/culturalHeritageConservation/IMA#objectType

ima:objectType rdf:type owl:DatatypeProperty ;
               
               rdfs:label "Object Type"@en ;
               
               dc:creator "Lidiya Dimitrova" ;
               
               skos:definition "Classification for the type of cultural object. This classification is supported by CMS (KeMU)"@en ;
               
               rdfs:domain chc:CulturalObject ;
               
               rdfs:range xsd:string .



###  http://www.sirma.com/ontologies/2016/02/culturalHeritageConservation/IMA#outsideDimensions

ima:outsideDimensions rdf:type owl:DatatypeProperty ;
                      
                      rdfs:label "Outside Dimensions"@en ;
                      
                      dc:creator "Lidiya Dimitrova" ;
                      
                      skos:definition "Outer dimension of the Frame (Text height and width)"@en ;
                      
                      rdfs:domain ima:Frame ;
                      
                      rdfs:range xsd:string .



###  http://www.sirma.com/ontologies/2016/02/culturalHeritageConservation/IMA#ownerNames

ima:ownerNames rdf:type owl:DatatypeProperty ;
               
               rdfs:label "Owner/Custodian"@en ;
               
               dc:creator "Lidiya Dimitrova" ;
               
               skos:definition "Owner of the Art Object."@en ;
               
               rdfs:domain chc:CulturalObject ;
               
               rdfs:range xsd:string .



###  http://www.sirma.com/ontologies/2016/02/culturalHeritageConservation/IMA#paintLayersDescription

ima:paintLayersDescription rdf:type owl:DatatypeProperty ;
                           
                           rdfs:label "Paint Layers Description"@en ;
                           
                           dc:creator "Lidiya Dimitrova" ;
                           
                           skos:definition "Technical description of the paint layer or design construction."@en ;
                           
                           rdfs:domain ima:Painting ;
                           
                           rdfs:range xsd:string .



###  http://www.sirma.com/ontologies/2016/02/culturalHeritageConservation/IMA#photographMount

ima:photographMount rdf:type owl:DatatypeProperty ;
                    
                    rdfs:label "Mount/Base"@en ;
                    
                    dc:creator "Lidiya Dimitrova" ;
                    
                    skos:definition "Type of material the photograph is mounted to."@en ;
                    
                    rdfs:domain ima:Photograph ;
                    
                    rdfs:range xsd:string .



###  http://www.sirma.com/ontologies/2016/02/culturalHeritageConservation/IMA#physicalDimensions

ima:physicalDimensions rdf:type owl:DatatypeProperty ;
                       
                       rdfs:label "Physical Dimensions"@en ;
                       
                       dc:creator "Lidiya Dimitrova" ;
                       
                       skos:definition "The physical attributes of the object without matte and/or frame. Both US and metric. Can be complex with multi-component or 3-dimensional objects.
Includes weight and other measures of the physical attributes of objects and their components."@en ;
                       
                       rdfs:domain chc:CulturalObject ;
                       
                       rdfs:range xsd:string .



###  http://www.sirma.com/ontologies/2016/02/culturalHeritageConservation/IMA#physicalLocation

ima:physicalLocation rdf:type owl:DatatypeProperty ;
                     
                     rdfs:label "Physical Location"@en ;
                     
                     dc:creator "Lidiya Dimitrova" ;
                     
                     skos:definition "Physical location of the sample so that someone could lay their hands on such as drawer number"@en ;
                     
                     rdfs:domain chc:Sample ;
                     
                     rdfs:range xsd:string .



###  http://www.sirma.com/ontologies/2016/02/culturalHeritageConservation/IMA#portfolio

ima:portfolio rdf:type owl:DatatypeProperty ;
              
              rdfs:label "Portfolio/Series"@en ;
              
              skos:definition "Indication of a group of works of art created as a group"@en ;
              
              dc:creator "Lidiya Dimitrova" ;
              
              rdfs:domain chc:CulturalObject ;
              
              rdfs:range xsd:string .



###  http://www.sirma.com/ontologies/2016/02/culturalHeritageConservation/IMA#preparatoryLayer

ima:preparatoryLayer rdf:type owl:DatatypeProperty ;
                     
                     rdfs:label "Ground/Preparatory Layer"@en ;
                     
                     skos:definition "An additional preparation layer for the image"@en ;
                     
                     dc:creator "Lidiya Dimitrova" ;
                     
                     rdfs:domain chc:CulturalObject ;
                     
                     rdfs:range xsd:string .



###  http://www.sirma.com/ontologies/2016/02/culturalHeritageConservation/IMA#primarySupportDescription

ima:primarySupportDescription rdf:type owl:DatatypeProperty ;
                              
                              rdfs:label "Primary Support Description"@en ;
                              
                              dc:creator "Lidiya Dimitrova" ;
                              
                              skos:definition "Text description of the paper support.
In case of photograpt descrives the type of photosensitive material the image lies on."@en ;
                              
                              rdfs:domain chc:CulturalObject ;
                              
                              rdfs:range xsd:string .



###  http://www.sirma.com/ontologies/2016/02/culturalHeritageConservation/IMA#primingDescription

ima:primingDescription rdf:type owl:DatatypeProperty ;
                       
                       rdfs:label "Sizing and Ground Description"@en ;
                       
                       dc:creator "Lidiya Dimitrova" ;
                       
                       skos:definition "Technical description of the sizing and ground construction"@en ;
                       
                       rdfs:domain ima:Painting ;
                       
                       rdfs:range xsd:string .



###  http://www.sirma.com/ontologies/2016/02/culturalHeritageConservation/IMA#rabbetDepth

ima:rabbetDepth rdf:type owl:DatatypeProperty ;
                
                rdfs:label "Rabbet Depth"@en ;
                
                skos:definition "How deep is the cavity where the artwork sits"@en ;
                
                dc:creator "Lidiya Dimitrova" ;
                
                rdfs:domain ima:Frame ;
                
                rdfs:range xsd:string .



###  http://www.sirma.com/ontologies/2016/02/culturalHeritageConservation/IMA#sampleSite

ima:sampleSite rdf:type owl:DatatypeProperty ;
               
               rdfs:label "Sample site"@en ;
               
               dc:creator "Lidiya Dimitrova" ;
               
               skos:definition "Location of the spot where the sample was taken: coordinates \"up\" and \"left\" or \"from right hand of the Litter\""@en ;
               
               rdfs:domain chc:Sample ;
               
               rdfs:range xsd:string .



###  http://www.sirma.com/ontologies/2016/02/culturalHeritageConservation/IMA#samplingDate

ima:samplingDate rdf:type owl:DatatypeProperty ;
                 
                 rdfs:label "Date taken"@en ;
                 
                 dc:creator "Lidiya Dimitrova" ;
                 
                 skos:definition "Date on which the sample was taken"@en ;
                 
                 rdfs:domain chc:Sample ;
                 
                 rdfs:range xsd:dateTime .



###  http://www.sirma.com/ontologies/2016/02/culturalHeritageConservation/IMA#secondarySupportDescription

ima:secondarySupportDescription rdf:type owl:DatatypeProperty ;
                                
                                rdfs:label "Secondary Support Description"@en ;
                                
                                dc:creator "Lidiya Dimitrova" ;
                                
                                skos:definition "Text description of any secondary support, example: thick laid paper, or the type of material the mount/base is attached to for photographs.."@en ;
                                
                                rdfs:domain chc:CulturalObject ;
                                
                                rdfs:range xsd:string .



###  http://www.sirma.com/ontologies/2016/02/culturalHeritageConservation/IMA#shape

ima:shape rdf:type owl:DatatypeProperty ;
          
          rdfs:label "Shape"@en ;
          
          dc:creator "Lidiya Dimitrova" ;
          
          skos:definition "Shape of the Frame"@en ;
          
          rdfs:domain ima:Frame ;
          
          rdfs:range xsd:string .



###  http://www.sirma.com/ontologies/2016/02/culturalHeritageConservation/IMA#sightSize

ima:sightSize rdf:type owl:DatatypeProperty ;
              
              rdfs:label "Sight Size"@en ;
              
              dc:creator "Lidiya Dimitrova" ;
              
              skos:definition "This is the size of the opening from the front of the frame.  "@en ;
              
              rdfs:domain ima:Frame ;
              
              rdfs:range xsd:string .



###  http://www.sirma.com/ontologies/2016/02/culturalHeritageConservation/IMA#specialConcerns

ima:specialConcerns rdf:type owl:DatatypeProperty ;
                    
                    rdfs:label "Special Concerns"@en ;
                    
                    skos:definition "Emphasized information (\"flag\") for the immediate attention of conservators or other staff members that the cultural object has conservation issues that impact its ability to be displayed"@en ;
                    
                    dc:creator "Lidiya Dimitrova"@en ;
                    
                    rdfs:range xsd:string .



###  http://www.sirma.com/ontologies/2016/02/culturalHeritageConservation/IMA#storageRequirement

ima:storageRequirement rdf:type owl:DatatypeProperty ;
                       
                       rdfs:label "Storage Requirement"@en ;
                       
                       skos:definition "Description on the storage requirements - wehether to store the piece flat, on a special hanger or other requirements."@en ;
                       
                       dc:creator "Lidiya Dimitrova"@en ;
                       
                       rdfs:range xsd:string .



###  http://www.sirma.com/ontologies/2016/02/culturalHeritageConservation/IMA#structuralPriority

ima:structuralPriority rdf:type owl:DatatypeProperty ;
                       
                       rdfs:label "Structural Priority"@en ;
                       
                       dc:creator "Lidiya Dimitrova"@en ;
                       
                       skos:definition "Structural stability determines priority for treatment"@en ;
                       
                       rdfs:domain chc:CulturalObject ;
                       
                       rdfs:range xsd:string .



###  http://www.sirma.com/ontologies/2016/02/culturalHeritageConservation/IMA#structureDescription

ima:structureDescription rdf:type owl:DatatypeProperty ;
                         
                         rdfs:label "Structure"@en ;
                         
                         dc:creator "Lidiya Dimitrova"@en ;
                         
                         skos:definition "The material used and the relationship between them."@en ;
                         
                         rdfs:domain chc:CulturalObject ;
                         
                         rdfs:range xsd:string .



###  http://www.sirma.com/ontologies/2016/02/culturalHeritageConservation/IMA#style

ima:style rdf:type owl:DatatypeProperty ;
          
          rdfs:label "Style"@en ;
          
          skos:definition "A way of Painting, drawing, building, composing, etc. Characteristic of a particular period, place, person or movement."@en ;
          
          dc:creator "Lidiya Dimitrova"@en ;
          
          rdfs:domain ima:Frame ;
          
          rdfs:range xsd:string .



###  http://www.sirma.com/ontologies/2016/02/culturalHeritageConservation/IMA#subClassification

ima:subClassification rdf:type owl:DatatypeProperty ;
                      
                      rdfs:label "Sub-Classification"@en ;
                      
                      skos:definition "Defines if the sample is whether from a cultural object or from a commercial material used in the conservation of the cultural object."@en ;
                      
                      dc:creator "Lidiya Dimitrova"@en ;
                      
                      rdfs:domain chc:Sample ;
                      
                      rdfs:range xsd:string .



###  http://www.sirma.com/ontologies/2016/02/culturalHeritageConservation/IMA#substrateDescription

ima:substrateDescription rdf:type owl:DatatypeProperty ;
                         
                         rdfs:label "Substrate Description"@en ;
                         
                         skos:definition "A substance or layer that underlies something, or on which some process occurs, in particular."@en ;
                         
                         dc:creator "Lidiya Dimitrova"@en ;
                         
                         rdfs:domain chc:CulturalObject ;
                         
                         rdfs:range xsd:string .



###  http://www.sirma.com/ontologies/2016/02/culturalHeritageConservation/IMA#supportDescription

ima:supportDescription rdf:type owl:DatatypeProperty ;
                       
                       rdfs:label "Support Description"@en ;
                       
                       skos:definition "A thing that bears the weight of something or keeps it upright."@en ;
                       
                       dc:creator "Lidiya Dimitrova"@en ;
                       
                       rdfs:domain chc:CulturalObject ;
                       
                       rdfs:range xsd:string .



###  http://www.sirma.com/ontologies/2016/02/culturalHeritageConservation/IMA#surfaceCoatingDescription

ima:surfaceCoatingDescription rdf:type owl:DatatypeProperty ;
                              
                              rdfs:label "Surface Coating Description"@en ;
                              
                              dc:creator "Lidiya Dimitrova"@en ;
                              
                              skos:definition "Technical description of the surface coating material"@en ;
                              
                              rdfs:domain ima:Painting ;
                              
                              rdfs:range xsd:string .



###  http://www.sirma.com/ontologies/2016/02/culturalHeritageConservation/IMA#surfaceDescription

ima:surfaceDescription rdf:type owl:DatatypeProperty ;
                       
                       rdfs:label "Surface Description"@en ;
                       
                       dc:creator "Lidiya Dimitrova"@en ;
                       
                       skos:definition "The outside part or uppermost layer of something (often used when describing its texture, form, or extent)."@en ;
                       
                       rdfs:domain chc:CulturalObject ;
                       
                       rdfs:range xsd:string .



###  http://www.sirma.com/ontologies/2016/02/culturalHeritageConservation/IMA#treatmentStage

ima:treatmentStage rdf:type owl:DatatypeProperty ;
                   
                   rdfs:label "Treatment phase"@en ;
                   
                   dc:creator "Lidiya Dimitrova"@en ;
                   
                   skos:definition "The treatment phase when the image was shot"@en ;
                   
                   rdfs:domain emf:Image ;
                   
                   rdfs:range xsd:string .



###  http://www.sirma.com/ontologies/2016/02/culturalHeritageConservation/IMA#variableComponents

ima:variableComponents rdf:type owl:DatatypeProperty ;
                       
                       rdfs:label "Variable Components"@en ;
                       
                       dc:creator "Lidiya Dimitrova"@en ;
                       
                       skos:definition "These are components that may be changed, or may not be included in a given installation"@en ;
                       
                       rdfs:domain chc:CulturalObject ;
                       
                       rdfs:range xsd:string .



###  http://www.sirma.com/ontologies/2016/02/culturalHeritageConservation/IMA#vendorNames

ima:vendorNames rdf:type owl:DatatypeProperty ;
                
                rdfs:label "Vendor/Vendor Manufacturer"@en ;
                
                dc:creator "Lidiya Dimitrova"@en ;
                
                skos:definition "The name of the Vendor who sold us the Frame."@en ;
                
                rdfs:domain ima:Frame ;
                
                rdfs:range xsd:string .



###  http://www.sirma.com/ontologies/2016/02/culturalHeritageConservation/IMA#watermarks

ima:watermarks rdf:type owl:DatatypeProperty ;
               
               rdfs:label "Watermarks"@en ;
               
               skos:definition "Free text description of any watermarks evident in the paper/support"@en ;
               
               dc:creator "Lidiya Dimitrova"@en ;
               
               rdfs:domain chc:CulturalObject ;
               
               rdfs:range xsd:string .





#################################################################
#
#    Classes
#
#################################################################


###  http://www.sirma.com/ontologies/2016/02/culturalHeritageConservation#Sample

chc:Sample emf:isCreateable "true"^^xsd:boolean ;
           
           emf:isPartOfObjectLibrary "true"^^xsd:boolean ;
           
           emf:isSearchable "true"^^xsd:boolean .



###  http://www.sirma.com/ontologies/2016/02/culturalHeritageConservation/IMA#BuiltEnvironment

ima:BuiltEnvironment rdf:type owl:Class ;
                     
                     rdfs:label "Built Environment"@en ;
                     
                     rdfs:subClassOf chc:CulturalObject ;
                     
                     emf:isCreateable "true"^^xsd:boolean ;
                     
                     emf:isSearchable "true"^^xsd:boolean ;
                     
                     emf:isPartOfObjectLibrary "true"^^xsd:boolean ;
                     
                     dc:creator "Lidiya Dimitrova"@en ;
                     
                     skos:definition "This record type includes the built and natural environment, covering constructed works and natural landscapes, forming a continuum from the largest natural landscapes and settled areas to the smallest of individual built works."@en .



###  http://www.sirma.com/ontologies/2016/02/culturalHeritageConservation/IMA#CeremonialEquipment

ima:CeremonialEquipment rdf:type owl:Class ;
                        
                        rdfs:label "Ceremonial Equipment"@en ;
                        
                        rdfs:subClassOf chc:CulturalObject ;
                        
                        emf:isCreateable "true"^^xsd:boolean ;
                        
                        emf:isPartOfObjectLibrary "true"^^xsd:boolean ;
                        
                        emf:isSearchable "true"^^xsd:boolean ;
                        
                        skos:definition "Articles or physical resources used to equip a person or thing, such as the instruments used in an activity or operation, which relate to or are used for ritual observances and formal events of a religious, societal, military, or public nature."@en ;
                        
                        dc:creator "Lidiya Dimitrova"@en .



###  http://www.sirma.com/ontologies/2016/02/culturalHeritageConservation/IMA#Container

ima:Container rdf:type owl:Class ;
              
              rdfs:label "Containers"@en ;
              
              rdfs:subClassOf chc:CulturalObject ;
              
              emf:isPartOfObjectLibrary "true"^^xsd:boolean ;
              
              emf:isSearchable "true"^^xsd:boolean ;
              
              emf:isCreateable "true"^^xsd:boolean ;
              
              dc:creator "Lidiya Dimitrova"@en ;
              
              skos:definition "This record type contains descriptors for artifacts used to hold substances or objects. Included are descriptors for containers intended for culinary use, for horticultural use, for health care, hygiene, and similar personal needs as well as descriptors for containers associated with liturgical, funerary, and other ceremonial activities. Curatorial Department will determine whether it is Decorative Art, Design Art, Ethnographic Art, Asian (i.e. Chinese, Japanese, Korean), etc."@en .



###  http://www.sirma.com/ontologies/2016/02/culturalHeritageConservation/IMA#Costume

ima:Costume rdf:type owl:Class ;
            
            rdfs:label "Costume"@en ;
            
            rdfs:subClassOf chc:CulturalObject ;
            
            emf:isSearchable "true"^^xsd:boolean ;
            
            emf:isPartOfObjectLibrary "true"^^xsd:boolean ;
            
            emf:isCreateable "true"^^xsd:boolean ;
            
            dc:creator "Lidiya Dimitrova"@en ;
            
            skos:definition "This record type contains descriptors for objects worn or carried for warmth, protection, embellishment, or for symbolic purposes. It includes descriptors for garments considered as the main item of dress (e.g., \"shirts,\" \"trousers\"), descriptors for garments worn under the main garments (e.g., \"undershirts\"), and descriptors for garments worn over the main garments (e.g., \"parkas\").  Also included are descriptors for protective wear, including types of armor; vestments and other ceremonial garments; uniforms. "@en .



###  http://www.sirma.com/ontologies/2016/02/culturalHeritageConservation/IMA#CostumeAccessory

ima:CostumeAccessory rdf:type owl:Class ;
                     
                     rdfs:label "Costume Accessory"@en ;
                     
                     rdfs:subClassOf chc:CulturalObject ;
                     
                     emf:isSearchable "true"^^xsd:boolean ;
                     
                     emf:isPartOfObjectLibrary "true"^^xsd:boolean ;
                     
                     emf:isCreateable "true"^^xsd:boolean ;
                     
                     skos:definition "Items that do not form the primary articles of clothing, but are instead the smaller articles of dress, such as shoes, gloves, hats, jewelry, etc.  (Mode of fashion)."@en ;
                     
                     dc:creator "Lidiya Dimitrova"@en .



###  http://www.sirma.com/ontologies/2016/02/culturalHeritageConservation/IMA#Drawing

ima:Drawing rdf:type owl:Class ;
            
            rdfs:label "Drawing"@en ;
            
            rdfs:subClassOf chc:CulturalObject ;
            
            emf:isSearchable "true"^^xsd:boolean ;
            
            emf:isCreateable "true"^^xsd:boolean ;
            
            emf:isPartOfObjectLibrary "true"^^xsd:boolean ;
            
            dc:creator "Lidiya Dimitrova"@en ;
            
            skos:definition "Visual works produced by drawing, which is the application of lines on a surface, often paper, by using a pencil, pen, chalk, or some other tracing instrument to focus on the delineation of form rather than the application of color. (Getty AAT)"@en .



###  http://www.sirma.com/ontologies/2016/02/culturalHeritageConservation/IMA#Frame

ima:Frame rdf:type owl:Class ;
          
          rdfs:label "Frame"@en ;
          
          rdfs:subClassOf chc:CulturalObject ;
          
          emf:isSearchable "true"^^xsd:boolean ;
          
          emf:isPartOfObjectLibrary "true"^^xsd:boolean ;
          
          emf:isCreateable "true"^^xsd:boolean ;
          
          skos:definition "Cases or structures that surround or enclose such items as works of art,mirrors, or documents, serving as support or protection or to call attention, while leaving the items visible."@en ;
          
          dc:creator "Lidiya Dimitrova"@en .



###  http://www.sirma.com/ontologies/2016/02/culturalHeritageConservation/IMA#Furnishing

ima:Furnishing rdf:type owl:Class ;
               
               rdfs:label "Furnishing"@en ;
               
               rdfs:subClassOf chc:CulturalObject ;
               
               emf:isPartOfObjectLibrary "true"^^xsd:boolean ;
               
               emf:isCreateable "true"^^xsd:boolean ;
               
               emf:isSearchable "true"^^xsd:boolean ;
               
               dc:creator "Lidiya Dimitrova"@en ;
               
               skos:definition """This record type contains descriptors for primarily movable articles that provide comfort, convenience, or protection in dwellings, places or business, or other public or private spaces. They may be useful or ornamental and may be used in indoor or outdoor spaces. (Sub-classifications can include: Decorative Arts such as furniture, seating furniture (chairs), table, desk, bed; and Textiles such as rugs, bedcovers, quilts, tapestries). Curatorial Department will determine whether it is Decorative Art, Design Art, Ethnographic Art, Asian (i.e. Chinese, Japanese, Korean), etc.

- Trade names and proper names for particular types of furnishing that have come to be used generically or near-generically are included in the hierarchy
- Objects whose primary purpose is to serve as storage receptacles or other forms of container (e.g., \"candle boxes\", \"footlockers\") appear in the Containers hierarchy. """@en .



###  http://www.sirma.com/ontologies/2016/02/culturalHeritageConservation/IMA#Multimedia

ima:Multimedia rdf:type owl:Class ;
               
               rdfs:label "Multimedia"@en ;
               
               rdfs:subClassOf chc:CulturalObject ;
               
               emf:isPartOfObjectLibrary "true"^^xsd:boolean ;
               
               emf:isSearchable "true"^^xsd:boolean ;
               
               emf:isCreateable "true"^^xsd:boolean ;
               
               skos:definition "Contemporary works of art that employ several distinct art forms, such as sculpture and music or painting and light art. Includes time- based and variable art."@en ;
               
               dc:creator "Lidiya Dimitrova"@en .



###  http://www.sirma.com/ontologies/2016/02/culturalHeritageConservation/IMA#Needlework

ima:Needlework rdf:type owl:Class ;
               
               rdfs:label "Needlework"@en ;
               
               rdfs:subClassOf chc:CulturalObject ;
               
               emf:isPartOfObjectLibrary "true"^^xsd:boolean ;
               
               emf:isSearchable "true"^^xsd:boolean ;
               
               emf:isCreateable "true"^^xsd:boolean ;
               
               dc:creator "Lidiya Dimitrova"@en ;
               
               skos:definition "Refers to works done with one or more needles and thread, yarn or cord. The term generally refers to work done by hand. Needlework includes sewing, embroidery, knitting, and other works. Until the 20th century \"plain sewing\" was the most widely practiced form of needlework in Western cultures. Most females learned basic sewing and knitting, which was used in the construction of clothing and the finishing of household textiles. With the introduction of machine sewing, needlework done by hand was often limited to decorative work."@en .



###  http://www.sirma.com/ontologies/2016/02/culturalHeritageConservation/IMA#Painting

ima:Painting rdf:type owl:Class ;
             
             rdfs:label "Painting"@en ;
             
             rdfs:subClassOf chc:CulturalObject ;
             
             emf:isSearchable "true"^^xsd:boolean ;
             
             emf:isPartOfObjectLibrary "true"^^xsd:boolean ;
             
             emf:isCreateable "true"^^xsd:boolean ;
             
             dc:creator "Lidiya Dimitrova"@en ;
             
             skos:definition "Unique works in which images are formed primarily by the direct application of pigments suspended in oil, water, egg yolk, molten wax, or other liquid, arranged in masses of color, onto a generally two-dimensional surface."@en .



###  http://www.sirma.com/ontologies/2016/02/culturalHeritageConservation/IMA#Pastel

ima:Pastel rdf:type owl:Class ;
           
           rdfs:label "Pastel"@en ;
           
           rdfs:subClassOf chc:CulturalObject ;
           
           emf:isPartOfObjectLibrary "true"^^xsd:boolean ;
           
           emf:isSearchable "true"^^xsd:boolean ;
           
           emf:isCreateable "true"^^xsd:boolean ;
           
           dc:creator "Lidiya Dimitrova"@en ;
           
           skos:definition "Works of art, typically on a paper or vellum support, to which designs are applied using crayons made of ground pigment held together with a binder, typically oil or water and gum. Works in this medium are sometimes classified as drawings, and sometimes as paintings, typically based on the local curatorial department responsible for the work or on the material of the support (pastels on paper may be classified as drawings, while pastels on vellum may be classified as paintings)."@en .



###  http://www.sirma.com/ontologies/2016/02/culturalHeritageConservation/IMA#Performance

ima:Performance rdf:type owl:Class ;
                
                rdfs:label "Performance"@en ;
                
                rdfs:subClassOf chc:CulturalObject ;
                
                emf:isPartOfObjectLibrary "true"^^xsd:boolean ;
                
                emf:isSearchable "true"^^xsd:boolean ;
                
                emf:isCreateable "true"^^xsd:boolean ;
                
                dc:creator "Lidiya Dimitrova"@en ;
                
                skos:definition "Refers to works of art that unfold over time and that combine elements of theater and object-oriented art."@en .



###  http://www.sirma.com/ontologies/2016/02/culturalHeritageConservation/IMA#Photograph

ima:Photograph rdf:type owl:Class ;
               
               rdfs:label "Photograph"@en ;
               
               rdfs:subClassOf chc:CulturalObject ;
               
               emf:isSearchable "true"^^xsd:boolean ;
               
               emf:isPartOfObjectLibrary "true"^^xsd:boolean ;
               
               emf:isCreateable "true"^^xsd:boolean ;
               
               dc:creator "Lidiya Dimitrova"@en ;
               
               skos:definition "Refers to still images produced from radiation-sensitive materials (sensitive to light, electron beams, or nuclear radiation), generally by means of the chemical action of light on a sensitive film, paper, glass, or metal. It does not include reproductive prints of documents and technical drawings.  Photographs may be positive or negative, opaque or transparent."@en .



###  http://www.sirma.com/ontologies/2016/02/culturalHeritageConservation/IMA#Print

ima:Print rdf:type owl:Class ;
          
          rdfs:label "Print"@en ;
          
          rdfs:subClassOf chc:CulturalObject ;
          
          emf:isCreateable "true"^^xsd:boolean ;
          
          emf:isPartOfObjectLibrary "true"^^xsd:boolean ;
          
          emf:isSearchable "true"^^xsd:boolean ;
          
          dc:creator "Lidiya Dimitrova"@en ;
          
          skos:definition "Pictorial works produced by transferring images by means of a matrix such as a plate, block, or screen, using any of various printing processes."@en .



###  http://www.sirma.com/ontologies/2016/02/culturalHeritageConservation/IMA#Sculpture

ima:Sculpture rdf:type owl:Class ;
              
              rdfs:label "Sculpture"@en ;
              
              rdfs:subClassOf chc:CulturalObject ;
              
              emf:isPartOfObjectLibrary "true"^^xsd:boolean ;
              
              emf:isSearchable "true"^^xsd:boolean ;
              
              emf:isCreateable "true"^^xsd:boolean ;
              
              dc:creator "Lidiya Dimitrova"@en ;
              
              skos:definition "Three-dimensional works of art in which images and forms are produced in relief, in intaglio, or in the round. The term refers particularly to art works created by carving or engraving a hard material, by molding or casting a malleable material (which usually then hardens), or by assembling parts to create a three-dimensional object. It is typically used to refer to large or medium-sized objects made of stone, wood, bronze, or another metal. Small objects are typically referred to as \"carvings\" or another appropriate term. \"Sculpture\" refers to works that represent tangible beings, objects, or groups of objects, or are abstract works that have defined edges and boundaries and can be measured."@en .



###  http://www.sirma.com/ontologies/2016/02/culturalHeritageConservation/IMA#Weapons

ima:Weapons rdf:type owl:Class ;
            
            rdfs:label "Weapons and Ammunition"@en ;
            
            rdfs:subClassOf chc:CulturalObject ;
            
            emf:isPartOfObjectLibrary "true"^^xsd:boolean ;
            
            emf:isCreateable "true"^^xsd:boolean ;
            
            emf:isSearchable "true"^^xsd:boolean ;
            
            dc:creator "Lidiya Dimitrova"@en ;
            
            skos:definition "This record type contains descriptors for implements and mechanisms designed to be used as a means of physical attack or defense. Included are hand-held weapons such as \"swords\", components of weapons (e.g., \"arrowheads\"), and objects propelled by firearms (e.g., \"cartridges\"). Also included are descriptors for hunting weapons (e.g., \"boar spears\") and for objects derived from weapons but used for purely ceremonial purposes (e.g., \"dress swords\"). The Curatorial Department will determine whether it is Ethnographic, Native American, Asian, etc."@en .





#################################################################
#
#    Annotations
#
#################################################################

chc:CulturalObject emf:isSearchable "true"^^xsd:boolean .


chc:documents emf:isSearchable "true"^^xsd:boolean .



chc:isDocumentedIn emf:isSearchable "true"^^xsd:boolean .



chc:hasDepiction emf:isSearchable "true"^^xsd:boolean .



emf:isPrimaryImageOf emf:isSearchable "true"^^xsd:boolean .



chc:hasParticipant emf:isSearchable "true"^^xsd:boolean .



chc:participates emf:isSearchable "true"^^xsd:boolean .



chc:hasAuthor emf:isSearchable "true"^^xsd:boolean .



chc:attachmentOf emf:isSearchable "true"^^xsd:boolean .



chc:hasAttachment emf:isSearchable "true"^^xsd:boolean .



chc:depicts emf:isSearchable "true"^^xsd:boolean .



chc:isCoauthorOf emf:isSearchable "true"^^xsd:boolean .



ptop:involvedIn emf:isSearchable "true"^^xsd:boolean .



chc:isParticipantIn emf:isSearchable "true"^^xsd:boolean .



chc:involves emf:isSearchable "true"^^xsd:boolean .



emf:processedBy emf:isSearchable "true"^^xsd:boolean .



chc:isAuthorOf emf:isSearchable "true"^^xsd:boolean .



chc:hasSupervisor emf:isSearchable "true"^^xsd:boolean .



chc:hasSample emf:isSearchable "true"^^xsd:boolean .



chc:isTakenFrom emf:isSearchable "true"^^xsd:boolean .



chc:ConservationActivity emf:isCreateable "true"^^xsd:boolean ;
                         
                         emf:isPartOfObjectLibrary "true"^^xsd:boolean ;
                         
                         emf:isSearchable "true"^^xsd:boolean .



emf:hasPrimaryImage emf:isSearchable "true"^^xsd:boolean .



chc:isSupervisorOf emf:isSearchable "true"^^xsd:boolean .



emf:processes emf:isSearchable "true"^^xsd:boolean .



ptop:hasParticipant emf:isSearchable "true"^^xsd:boolean .



chc:hasCoauthor emf:isSearchable "true"^^xsd:boolean .




###  Generated by the OWL API (version 3.4.2) http://owlapi.sourceforge.net

